src/high/weakestpre/at/alloc.v
@@ -1,0 +1,450 @@
+From iris.proofmode Require Import proofmode monpred.
+From iris.algebra Require Import gset.
+From iris_named_props Require Import named_props.
+
+From self Require Import extra solve_view_le encode_relation map_extra view_slice ipm_tactics.
+
+From self.lang Require Import syntax tactics lemmas.
+
+From self.base Require Import generational_resources primitive_laws.
+
+From self.high Require Import wrappers monpred_simpl protocol locations crash_weakestpre weakestpre.
+From self.high.modalities Require Import post_fence_sync_advanced.
+From self.high.lib Require Import abstract_state increasing_map.
+
+From self Require Export lang.
+From self.high Require Export dprop.
+
+Set Default Proof Using "Type*".
+
+Section wp_at_alloc.
+  Context `{AbstractState ST}.
+  Context `{!nvmBaseGS Σ Ω, !nvmHighGS Σ Ω, PerennialG Σ}.
+
+  Implicit Types (ℓ : loc) (σ : ST) (prot : LocationProtocol ST).
+
+  (** * Shared points-to predicate *)
+
+  Lemma msg_persisted_views_eq
+        (ℓ : loc) (hists : gmap loc (gmap time (message * positive)))
+        (hist : gmap time (message * positive)) (msg : message)
+        (atLocs : gset loc) (t : time) (s' : positive) γ :
+    map_Forall
+      (λ _ : loc,
+        map_Forall
+          (λ _ '(msg, _), msg_persist_view msg = msg_persisted_after_view msg))
+      (restrict atLocs hists) →
+    hists !! ℓ = Some hist →
+    hist !! t = Some (msg, s') →
+    gen_alocs_auth γ atLocs -∗
+    gen_alocs_frag γ {[ ℓ ]} -∗
+    ⌜msg.(msg_persist_view) = msg.(msg_persisted_after_view)⌝.
+  Proof.
+    iIntros (m look look') "A B".
+    iDestruct (location_sets_singleton_included with "A B") as %V.
+    iPureIntro.
+    assert (restrict atLocs hists !! ℓ = Some hist) as look2.
+    - apply restrict_lookup_Some. done.
+    - setoid_rewrite map_Forall_lookup in m.
+      specialize (m ℓ hist look2).
+      setoid_rewrite map_Forall_lookup in m.
+      specialize (m t (msg, s') look').
+      simpl in m.
+      done.
+  Qed.
+  
+  Lemma interp_insert_loc_at ℓ prot `{!ProtocolConditions prot} s SV PV BV v :
+    SV !!0 ℓ = 0 →
+    interp -∗
+    p_full prot s v (SV, PV, BV) -∗
+    p_pers prot s v (SV, PV, BV) -∗
+    (* persisted {[ ℓ := MaxNat 0 ]} -∗ *)
+    ℓ ↦fh initial_history AT SV PV v ==∗
+    (ℓ ↦_AT^{prot} [s]) (SV, PV, BV) ∗ interp.
+  Proof.
+    iIntros (svLook).
+    iNamed 1.
+    iIntros "predFull predPers pts".
+
+    (* The new location is not in the existing [phys_hist]. *)
+    destruct (phys_hists !! ℓ) eqn:physHistsLook.
+    { assert (is_Some (offsets !! ℓ)) as (? & ?).
+      { apply elem_of_dom. rewrite -offsetsDom. apply elem_of_dom. done. }
+      iDestruct (big_sepM_lookup with "ptsMap") as "pts'".
+      { naive_solver. }
+      iDestruct (fmapsto_valid_2 with "pts pts'") as (?) "_".
+      done. }
+
+    iDestruct (big_sepM2_dom with "predsFullReadHold") as %domEq.
+    iDestruct (big_sepM2_dom with "bumperSome") as %domEq2.
+    iDestruct (big_sepM2_dom with "bumpMono") as %domEq4.
+
+    assert (offsets !! ℓ = None) as offsetsLook.
+    { apply not_elem_of_dom. rewrite -offsetsDom. apply not_elem_of_dom. done. }
+    assert (abs_hists !! ℓ = None) as absHistsLook.
+    { apply not_elem_of_dom. rewrite -domEq. apply not_elem_of_dom.
+      assumption. }
+    assert (ℓ ∉ dom abs_hists) as absHistsDomElem.
+    { apply not_elem_of_dom. done. }
+
+    (** We update ghost state. **)
+    (* add offset to offsets *)
+    iMod (offset_auth_insert with "offsets") as "[offsets #offset]".
+    { apply not_elem_of_dom. done. }
+    (* Allocate new physical history for the location. *)
+    iMod (auth_map_map_insert_top _ _ _ (initial_history AT SV PV v) with "physHists") as "[physHists #physHistFrag]".
+    { done. }
+
+    (* Add the predicate for the location. *)
+    iMod (own_all_preds_insert _ _ _ prot.(p_full) with "full_predicates") as "[full_predicates knowFullPred]".
+    { eapply map_dom_eq_lookup_None; last apply physHistsLook.
+      congruence. }
+    iMod (own_all_preds_insert _ _ _ prot.(p_read) with "read_predicates") as "[read_predicates knowReadPred]".
+    { eapply map_dom_eq_lookup_None; last apply physHistsLook.
+      congruence. }
+    iMod (own_all_preds_insert _ _ _ prot.(p_pers) with "pers_predicates") as "[pers_predicates knowPersPred]".
+    { eapply map_dom_eq_lookup_None; last apply physHistsLook.
+      congruence. }
+    
+    (* Unlike Spirea 1.0, the abstract history now depends on knowing the bumper first. *)
+    (* Add the bumper for the location. *)
+    iMod (own_all_bumpers_insert _ _ _ (prot.(p_bumper)) with "allBumpers")
+      as "[allBumpers #knowBumper]".
+    { eapply map_dom_eq_lookup_None; last apply physHistsLook. congruence. }
+    (* Allocate the abstract history for the location. *)
+    iMod (full_map_insert _ _ _ _ _ {[0 := encode s]} with "crashedRely [knowBumper] history")
+      as "(history & ownHist & #fragHist)".
+    { eapply map_dom_eq_lookup_None; last apply physHistsLook. congruence. }
+    { iDestruct "knowBumper" as "[? $]". }
+    iEval (rewrite big_sepM_singleton) in "fragHist".
+
+    (* Add the preorder for the location. (I don't know what) *)
+    iMod (ghost_map_insert_persist with "allOrders") as "[allOrders #knowOrder]".
+    { eapply map_dom_eq_lookup_None; last apply physHistsLook.
+      rewrite /relation2. congruence. }
+
+    (* Add the allocated location to the set of atomic locations. *)
+    iMod (gen_alocs_update _ ℓ with "atLocs") as "[atLocs #isAtLoc]".
+
+    iAssert (know_protocol ℓ prot (SV, PV, BV)) as "#prot".
+    { rewrite /know_protocol.
+      iEval (monPred_simpl).
+      rewrite !monPred_at_embed.
+      iFrame "knowFullPred knowReadPred knowPersPred knowBumper knowOrder". }
+
+    iModIntro.
+    iSplitL "knowFullPred knowReadPred knowPersPred knowBumper".
+    { rewrite /mapsto_at.
+      iExists _, {[ 0 := (Msg v SV PV PV) ]}, 0, 0, 0, s, _.
+      iSplitPure; first done.
+      iSplitPure; first apply map_extra.map_sequence_singleton.
+      iSplitPure; first apply map_sequence_singleton.
+      iSplitPure. { apply map_no_later_singleton. }
+      iSplitPure. { set_solver+. }
+      iSplit; first iAssumption.
+      iSplit; first iAssumption.
+      iSplitPure. { apply increasing_map_singleton. }
+      iEval (rewrite 2!big_sepM_singleton).
+      iDestruct (frag_history_equiv with "fragHist") as "$".
+      iFrame "physHistFrag".
+      simpl.
+      iSplitPure; first done.
+      iSplitL; last (iPureIntro; lia).
+      done. }
+    iExistsN.
+    iSplitL "ptsMap pts".
+    { iDestruct (big_sepM_insert with "[pts $ptsMap]") as "$"; done. }
+    iFrameNamedF.
+    iSplitPure; first set_solver.
+    iFrameNamedF.
+    iFrame "full_predicates read_predicates pers_predicates allOrders naLocs atLocs".
+
+    (* I couldn't figure out how to use [comm] typeclass. *)
+    replace (at_locs ∪ {[ ℓ ]}) with ({[ ℓ ]} ∪ at_locs); last set_solver.
+    
+    (* historyFragments *)
+    iSplit.
+    { iApply (big_sepM_insert_2 with "[] historyFragments");
+      simpl; rewrite big_sepM_singleton; iFrame "fragHist". }
+    (* locsDisjoint *)
+
+    iSplitPure. {
+      assert (ℓ ∉ dom abs_hists).
+      { rewrite -domEq. apply not_elem_of_dom. done. }
+      set_solver. }
+    (* histDomLocs *)
+    iSplitPure. { rewrite dom_insert_L. set_solver+ histDomLocs. }
+    (* naViewsDom *)
+    iSplitPure; first done.
+    iFrame "naView".
+    (* mapShared *)
+    iSplitPure.
+    { rewrite -map_insert_zip_with.
+      
+      rewrite restrict_insert_union.
+      rewrite /shared_locs_inv.
+      rewrite /map_map_Forall.
+      apply map_Forall_insert_2; last done.
+      rewrite /initial_history.
+      simpl.
+      rewrite drop_prefix_zero.
+      rewrite map_Forall_singleton.
+      done. }
+    iSplitL "atLocsHistories ownHist".
+    { rewrite restrict_insert_union big_sepM_insert.
+      2: { apply restrict_lookup_None_lookup. assumption. }
+      iFrame "ownHist atLocsHistories". }
+    (* "ordered" *)
+    iSplit.
+    { iApply (big_sepM2_insert_2); last done.
+      iPureIntro. apply increasing_map_singleton. }
+    (* histPViewDoms *)
+    iSplitPure.
+    { rewrite dom_insert.
+      apply union_subseteq_r', histPViewDoms. }
+    (* predsFullHold *)
+    iSplitL "predsFullReadHold predFull".
+    { iApply (big_sepM2_insert with "[predFull predsFullReadHold]").
+      { done. } { done. }
+      iSplitL "predFull".
+      - iExistsN. rewrite ?lookup_insert.
+        iSplitPure; first done.
+        iSplitPure; first done.
+        iSplitPure; first done.
+        rewrite /initial_history.
+        rewrite big_sepM2_singleton /=.
+        assert (na_views !! ℓ = None) as ->.
+        { apply not_elem_of_dom in physHistsLook.
+          apply not_elem_of_dom.
+          rewrite naViewsDom.
+          eapply not_elem_of_weaken; first apply physHistsLook.
+          rewrite domEq histDomLocs.
+          set_solver. }
+        simpl.
+        rewrite lookup_singleton_ne; last done.
+        destruct (decide _) as [ | contra ].
+        + iPoseProof (into_no_buffer_at with "predFull") as "predFull".
+          iApply (predicate_holds_phi_decode_2 with "[//] predFull").
+          apply decode_encode.
+        + exfalso.
+          by apply contra.
+      - iApply (big_sepM2_impl with "predsFullReadHold").
+        iIntros "!>" (ℓ' ????) "H".
+        assert (ℓ ≠ ℓ') by congruence.
+        iApply (encoded_full_read_predicates_hold_equiv with "H");
+          try (rewrite lookup_insert_ne; last done);
+          done. }
+    (* predsPersHold *)
+    iSplitL "predsPersHold predPers".
+    { iApply (big_sepM2_insert with "[predPers predsPersHold]").
+      { done. } { done. }
+      iSplitL "predPers".
+      - iExistsN. rewrite ?lookup_insert.
+        iSplitPure; first done.
+        iSplitPure; first done.
+        iSplitPure; first apply lookup_singleton.
+        iSplitPure; first done.
+        iSplitPure.
+        { rewrite /lookup_zero not_elem_of_dom_1 //. set_solver. }
+        iSplitL "".
+        { rewrite not_elem_of_dom_1 /= //. set_solver. }
+        iPoseProof (objective_at with "predPers") as "predPers".
+        iApply (predicate_holds_phi_decode_2 with "[//] predPers").
+        apply decode_encode.
+      - iApply (big_sepM2_impl with "predsPersHold").
+        iIntros "!>" (ℓ' ????) "H".
+        assert (ℓ ≠ ℓ') by congruence.
+        iApply (encoded_pers_predicate_holds_equiv with "H");
+          try (rewrite lookup_insert_ne; last done);
+          done. }
+    iFrame "allBumpers".
+    (* bumpMono *)
+    iSplit.
+    { iApply (big_sepM2_insert_2 with "[] bumpMono").
+      iPureIntro. simpl.
+      apply encode_bumper_bump_mono. apply bumper_mono. }
+    (* bumper = three domains *)
+    iSplitPure; first set_solver.
+    iSplitPure; first set_solver.
+    iSplitPure; first set_solver.
+    (* predPostCrash *)
+    (* iSplit. { *)
+    (*   iApply (big_sepM2_insert_2 with "[]"). *)
+    (*   - iExists _, _, _. *)
+    (*     rewrite ?lookup_insert. *)
+    (*     do 3 (iSplitPure; first done). *)
+    (*     iModIntro. iIntros (????) "(%P_pers & #eqPers & persHolds)". *)
+    (*     iSplit. *)
+    (*     + iIntros (???) "(%P_full & #eqFull & fullHolds) %bumperEq". *)
+    (*       apply encode_bumper_Some_decode in bumperEq. *)
+    (*       destruct bumperEq as (s3 & bumperEq & bumperEq'). *)
+    (*       iEval (rewrite /encode_predicate). *)
+    (*       rewrite -bumperEq'. *)
+    (*       rewrite decode_encode. *)
+    (*       iExists _, _. *)
+    (*       iSplit. { iPureIntro. simpl. reflexivity. } *)
+    (*       iSplit. { iPureIntro. simpl. reflexivity. } *)
+    (*       iDestruct (encode_predicate_decode with "eqPers") as (s4) "%s5DecodeEq". *)
+    (*       iPoseProof (encode_predicate_extract with "eqPers persHolds") as "predPers". *)
+    (*       { done. } *)
+    (*       iPoseProof (encode_predicate_extract with "eqFull fullHolds") as "predFull". *)
+    (*       { done. } *)
+    (*       iPoseProof (pred_full_post_crash with "predPers") as "[PostCrash _]". *)
+    (*       by iApply "PostCrash". *)
+    (*     + iIntros (??????) "#eqFull". *)
+    (*       iDestruct (encode_predicate_decode with "eqPers") as (s4) "%s4DecodeEq". *)
+    (*       iPoseProof (encode_predicate_extract with "eqPers persHolds") as "predPers". *)
+    (*       { done. } *)
+    (*       iDestruct (encode_predicate_decode with "eqFull") as (s5) "%s5DecodeEq". *)
+    (*       iPoseProof (pred_full_post_crash with "predPers") as "[_ PostCrash]". *)
+    (*       (* we need to instantiate the universal, but we cannot find the *)
+    (*          instance for [s_c], because we don't know whether [decode e_c] *)
+    (*          yields anything, not until after we instantiate [s_c]. but we can *)
+    (*          get around it by case distinction. *) *)
+    (*       destruct (@decode ST _ _ e_c) as [s3 | ] eqn:Heqn. *)
+    (*       * iDestruct ("PostCrash" $! s5 v_f s3 v_c) as (P_obj) "[objImpl PostCrash]". *)
+    (*         iExists P_obj. *)
+    (*         iSplitL "objImpl". { *)
+    (*           (* monPred_simpl. *) *)
+    (*           iIntros (?). *)
+    (*           rewrite monPred_at_wand. *)
+    (*           iIntros (view') "% fullHolds". *)
+    (*           iPoseProof (encode_predicate_extract with "eqFull fullHolds") as "predFull". *)
+    (*           { done. } *)
+    (*           iSpecialize ("objImpl" $! view' with "predFull"). *)
+    (*           iFrame. *)
+    (*         } *)
+    (*         iIntros "objHolds %bumperEq %order1 %order2 (%P_read & #eqRead & readHolds)". *)
+    (*         iSpecialize ("PostCrash" with "objHolds"). *)
+    (*         apply encode_bumper_Some_decode in bumperEq. *)
+    (*         destruct bumperEq as (s3' & bumperEq & bumperEq'). *)
+    (*         iEval (rewrite /encode_predicate). *)
+    (*         rewrite -bumperEq'. *)
+    (*         rewrite decode_encode. *)
+    (*         simplify_eq. *)
+    (*         iPoseProof (encode_predicate_extract with "eqRead readHolds") as "predRead". *)
+    (*         { done. } *)
+    (*         iPoseProof (monPred_wand_force with "PostCrash") as "PostCrash". *)
+    (*         iSpecialize ("PostCrash" with "predRead"). *)
+    (*         iExists _, _. *)
+    (*         iSplit. { iPureIntro. simpl. reflexivity. } *)
+    (*         iSplit. { iPureIntro. simpl. reflexivity. } *)
+    (*         rewrite encode_relation_decode_iff in order1; [ | done | done ]. *)
+    (*         rewrite encode_relation_decode_iff in order2; [ | done | done ]. *)
+    (*         iApply "PostCrash"; iPureIntro; destruct order1; simplify_eq; done. *)
+    (*       * (* this is the spurious case, we will see that once we get hold of *)
+    (*            [encode_bumper], we will just feed some random [ST] *) *)
+    (*         iDestruct ("PostCrash" $! s5 v_f s4 v_c) as (P_obj) "[objImpl PostCrash]". *)
+    (*         iExists P_obj. *)
+    (*         iSplitL "objImpl". { *)
+    (*           (* monPred_simpl. *) *)
+    (*           iIntros (?). *)
+    (*           rewrite monPred_at_wand. *)
+    (*           iIntros (view') "% fullHolds". *)
+    (*           iPoseProof (encode_predicate_extract with "eqFull fullHolds") as "predFull". *)
+    (*           { done. } *)
+    (*           iSpecialize ("objImpl" $! view' with "predFull"). *)
+    (*           iFrame. *)
+    (*         } *)
+    (*         iIntros "_ %bumperEq". *)
+    (*         apply encode_bumper_Some_decode in bumperEq. *)
+    (*         destruct bumperEq as (s3' & bumperEq & bumperEq'). *)
+    (*         rewrite Heqn in bumperEq. *)
+    (*         discriminate. *)
+    (*   - iApply (big_sepM2_impl with "predFullPostCrash"). *)
+    (*     iIntros "!> %ℓ' %pred_full %bumper %predFullLook %bumperLook *)
+    (*              (%pred_read & %pred_pers & %order & *)
+    (*               %predReadLook & %predPersLook & %orderLook & PostCrash)". *)
+    (*     iExists pred_read, pred_pers, order. *)
+    (*     assert (ℓ' ∈ dom abs_hists). { *)
+    (*       apply elem_of_dom_2 in bumperLook. *)
+    (*       congruence. *)
+    (*     } *)
+    (*     assert (ℓ ≠ ℓ') by congruence. *)
+    (*     do ? (rewrite lookup_insert_ne; last done). *)
+    (*     do 3 (iSplitPure; first done). *)
+    (*     iApply "PostCrash". *)
+    (* } *)
+    (* [read_nextgen] *)
+    iSplit. {
+      iApply (big_sepM2_insert_2 with "[] predReadNextgen").
+      iIntros (????) "%bumperEq".
+      iApply (plainly_intro emp); last done.
+      iIntros "_ (%Pread & #eqRead & ReadHolds)".
+      apply encode_bumper_Some_decode in bumperEq.
+      destruct bumperEq as (s3 & bumperEq & bumperEq').
+      iEval (rewrite /encode_predicate).
+      rewrite -bumperEq'.
+      rewrite decode_encode.
+      iExists _.
+      iSplit. { iPureIntro. simpl. reflexivity. }
+      iPoseProof (encode_predicate_extract with "eqRead ReadHolds") as "predRead".
+      { done. }
+      iPoseProof (pred_read_nextgen with "predRead") as "nextgen".
+      iApply "nextgen". }
+    (* [full_read_split] *)
+    iSplit. {
+      iApply (big_sepM2_insert_2 with "[] predFullReadSplit").
+      iIntros (???).
+      iApply (plainly_intro emp); last done.
+      iIntros "_ (%P_full & #eqFull & fullHolds)".
+      iDestruct (encode_predicate_decode with "eqFull") as (s4) "%s4DecodeEq".
+      iPoseProof (encode_predicate_extract with "eqFull fullHolds") as "predFull".
+      { done. }
+      iPoseProof (full_read_split with "predFull") as "[predRead _]".
+      iExists _.
+      iEval (rewrite /encode_predicate s4DecodeEq).
+      iSplit; done.
+    }
+    (* bumperBumpToValid *)
+    iSplitPure.
+    { rewrite map_Forall_insert.
+      2: { eapply map_dom_eq_lookup_None; last apply physHistsLook. congruence. }
+      split; last done.
+      apply encode_bumper_bump_to_valid. }
+    (* bumperSome *)
+    iApply (big_sepM2_insert_2 with "[] bumperSome").
+    iPureIntro.
+    apply map_Forall_singleton.
+    rewrite encode_bumper_encode.
+    done.
+  Qed.
+
+  Lemma wp_alloc_at v s prot `{!ProtocolConditions prot} st E :
+    {{{ prot.(p_full) s v ∗ prot.(p_pers) s v }}}
+      ref_AT v @ st; E
+    {{{ ℓ, RET #ℓ; ℓ ↦_AT^{prot} [s] }}}.
+  Proof.
+    intros Φ.
+    iModel.
+    iIntros "[ϕ_full ϕ_pers]".
+    iIntros (TV' incl) "Φpost".
+    iApply wp_unfold_at.
+    iIntros ([[SV PV] BV] incl2) "#val".
+    iApply wp_extra_state_interp. { done. } { by apply prim_step_ref_no_fork. }
+    iIntros "interp".
+    (* We add this to prevent Coq from trying to use [highExtraStateInterp]. *)
+    set (extra := (Build_extraStateInterp _ _)).
+    iApply (@program_logic.crash_weakestpre.wpc_wp).
+    iApply @wpc_fupd.
+    iApply @program_logic.crash_weakestpre.wp_wpc.
+    iApply (wp_alloc (extra := {| extra_state_interp := True |})); first done.
+    iNext.
+    iIntros (ℓ CV') "(crashedAt' & % & % & pts)".
+    simpl.
+    iFrame "val".
+    destruct TV as [[??]?].
+    iMod (interp_insert_loc_at ℓ prot _ _ _ BV with "interp [ϕ_full] [ϕ_pers] pts")
+      as "(pts & interp)"; first done.
+    { iApply monPred_mono; last iApply "ϕ_full". solve_view_le. }
+    { iApply monPred_mono; last iApply "ϕ_pers". solve_view_le. }
+    iModIntro.
+    rewrite -assoc. iSplit; first done.
+    iFrame "interp".
+    iSpecialize ("Φpost" $! ℓ).
+    monPred_simpl. 
+    iApply ("Φpost" with "[] pts").
+    { done. }
+  Qed.
+
+End wp_at_alloc.
