src/high/weakestpre/at/cas.v
@@ -1,0 +1,598 @@
+From iris.proofmode Require Import proofmode monpred.
+From iris.algebra Require Import gset.
+From iris_named_props Require Import named_props.
+
+From self Require Import extra solve_view_le encode_relation map_extra view_slice.
+
+From self.lang Require Import syntax tactics lemmas.
+
+From self.base Require Import generational_resources primitive_laws.
+
+From self.high Require Import wrappers monpred_simpl protocol locations crash_weakestpre weakestpre.
+From self.high.modalities Require Import post_fence_sync_advanced.
+From self.high.lib Require Import abstract_state increasing_map.
+From self.high.weakestpre.at Require Import prelude.
+
+From self Require Export lang.
+From self.high Require Export dprop.
+
+Set Default Proof Using "Type*".
+
+Section wp_at.
+  Context `{AbstractState ST}.
+  Context `{!nvmBaseGS Σ Ω, !nvmHighGS Σ Ω, PerennialG Σ}.
+
+  Implicit Types (ℓ : loc) (σ : ST) (prot : LocationProtocol ST).
+  
+  (** Variables:
+   * [σ_i] and [v_i]: the state and value we read last time.
+   * [σ_l] and [v_l]: the state and value we read this time.
+   * [σ_t] and [v_t]: the state and value we write if successful.
+   * [σ_n] and [v_n]: any other "dangling" state not on the main timeline (through write-only operations).
+   * [σ_p] and [v_p]: the pview state and value.
+   * [Q1]: the success postcondition.
+   * [Q2]: the failure postcondition.
+   * [Q3]: the failure postcondition outside of fence.
+   * [abs_hist'], [phys_hist']: observed history form the [mapsto_at] assertion.
+   * [abs_hist], [phys_hist]: complete history from [interp]. *)
+  Lemma wp_cmpxchg_at Q1 Q2 Q3 (P R: ST → dProp Σ) σs σ_i σ_t ℓ prot `{!ProtocolConditions prot} v_i v_t st E :
+    {{{
+      ℓ ↦_AT^{prot} (σs ++ [σ_i]) ∗
+      (∀ σ_l v_l σ_p v_p,
+        (* we know that we won't read older state than [σ_i] *)
+        ⌜ σ_i ⊑ σ_l ⌝ -∗
+        ((▷ prot.(p_read) σ_l v_l) -∗ ⌜ vals_compare_safe v_i v_l ⌝) ∗
+        (( (* in case of success *)
+            ⌜ v_l = v_i ⌝ -∗
+            (* The state we write fits in the history. *)
+            <obj> (prot.(p_full) σ_l v_l -∗ ⌜ σ_l ⊑ σ_t ⌝) ∗
+            (∀ σ_n v_n, ⌜ σ_l ⊑ σ_n ⌝ -∗ prot.(p_full) σ_l v_l -∗
+                        prot.(p_full) σ_n v_n ∨
+                        (prot.(p_read) σ_n v_n ∧
+                        ∃ σ_n' v_n', ⌜ σ_n ⊑ σ_n' ⌝ ∗ prot.(p_full) σ_n' v_n') -∗
+                        ⌜ σ_t ⊑ σ_n ⌝) ∗
+            (* Extract the objective knowledge from [p_pers] *)
+            <obj> (prot.(p_pers) σ_p v_p -∗ <obj> P σ_p ∗ (P σ_p -∗ prot.(p_pers) σ_p v_p)) ∗
+            (* Extract from the location we load. *)
+            <obj> (prot.(p_full) σ_l v_l ∗ P σ_p -∗ prot.(p_read) σ_l v_l ∗ R σ_l) ∗
+            (* Establish the invariant for the value we store. *)
+            (R σ_l ==∗ prot.(p_full) σ_t v_t ∗ <obj> P σ_p ∗ Q1 σ_l))
+         ∧ (* in case of failure *)
+           ((<obj> (prot.(p_full) σ_l v_l -∗ prot.(p_full) σ_l v_l ∗ Q2 σ_l)) ∗ Q3)
+        ))
+    }}}
+      CmpXchg #ℓ v_i v_t @ st; E
+    {{{ v b σ_l, RET (v, #b);
+      (⌜ b = true ⌝ ∗ <fence> Q1 σ_l ∗ ℓ ↦_AT^{prot} ((σs ++ [σ_i]) ++ [σ_t]) ∗ seen_state ℓ prot σ_l) ∨
+      (⌜ b = false ⌝ ∗ ⌜ σ_i ⊑ σ_l ⌝ ∗ ℓ ↦_AT^{prot} (σs ++ [σ_i]) ∗ <fence> (Q2 σ_l) ∗ Q3)
+    }}}.
+  Proof.
+    intros Φ.
+    iModel.
+    iIntros "(pts & impl)".
+
+    iDestruct "pts" as (abs_hist' phys_hist' tLo t_i offset σ' ms) "H". iNamed "H".
+    assert (σ' = σ_i) as -> by (rewrite last_snoc in lastEq; simplify_eq; done).
+    iDestruct "tSLe" as %tSLe.
+
+    (* We unfold the WP. *)
+    iIntros (TV' incl) "Φpost".
+    iApply wp_unfold_at.
+    iIntros ([[SV PV] BV] incl2) "#val".
+    iApply wp_extra_state_interp. { done. }
+    { apply prim_step_cmpxchg_no_fork. }
+
+    iIntros "interp".
+    iAssert (∃ OCV, crashed_at_offset OCV ∗ ⌜ OCV !!0 ℓ = offset ⌝)%I as (OCV) "[#offsets <-]".
+    { iDestruct "offset" as (?) "(? & ? & %)".
+      iExists _.
+      by iFrame "#". }
+    
+    iDestruct (interp_get_at_loc with "interp isAtLoc locationProtocol offset")
+      as (phys_hists phys_hist abs_hist encp_full encp_read encp_pers pview) "(R & reins)".
+    iNamed "R".
+
+    set (extra := (Build_extraStateInterp _ _)).
+    iApply (@program_logic.crash_weakestpre.wpc_wp).
+    iApply @wpc_fupd.
+    iApply @program_logic.crash_weakestpre.wp_wpc.
+
+    assert (abs_hist' !! t_i = Some σ_i).
+    { eapply map_sequence_lookup_hi in slice.
+      rewrite last_snoc in slice.
+      apply slice. }
+
+    rewrite ?monPred_at_big_sepM.
+    iDestruct (big_sepM_lookup with "absHist") as "hist"; first done.
+    iEval (rewrite monPred_at_embed) in "hist".
+    iDestruct (history_full_entry_frag_lookup with "fullHist hist")
+      as %(encσ_i & Hlookσ_i & Hdecodeσ_i).
+
+    iApply (wp_cmpxchg_alt with "[#] [$offsets $pts $val]").
+    (* [val_safe_compare] proof *)
+    { iIntros (t_l [v_l SV_l PV_l BV_l] leT physHistLook).
+      simpl in leT.
+
+      assert (store_view TV !!0 ℓ ≤ SV !!0 ℓ).
+      { f_equiv. solve_view_le. }
+      assert (t_i ≤ t_l) as le by lia.
+
+      eassert _ as  temp. { eapply (read_atomic_location t_i t_l (OCV !!0 ℓ)); (done || lia). }
+      destruct temp as (σ_l & encσ_l & ? & ? & ? & <- & orderRelated).
+
+      iDestruct ("impl" $! _ v_l _ _ orderRelated) as "(safe & _)".
+      iEval (monPred_simpl) in "safe".
+      iEval (setoid_rewrite monPred_at_pure) in "safe".
+      iApply ("safe" $! (TV ⊔ (SV_l, PV_l, ∅)) with "[%]"); first solve_view_le.
+
+      iDestruct (big_sepM2_lookup _ _ _ t_l with "predFullReadHolds") as "predFR". 
+      { done. } { done. }
+      simpl.
+      iAssert (encoded_predicate_holds encp_read encσ_l v_l (SV_l, PV_l, ∅))%I
+        with "[predFR]" as "predR".
+      { destruct (decide (_)).
+        - iDestruct ("predFullReadSplit" with "predFR") as "$".
+        - iApply "predFR". }
+      
+      iNext.
+      iDestruct (predicate_holds_phi_decode with "predReadEquiv predR") as "predR";
+        first done.
+      iApply monPred_mono; last iApply "predR".
+      solve_view_le. }
+    iEval (simpl).
+    iIntros "!>" (t_l v_l SV_l FV_l PV_l SV_t succ) "(%le & #valT & % & % & disj)".
+    iFrame "valT".
+    iDestruct "disj" as "[H | H]".
+    - (* success *)
+      iDestruct "H" as "(-> & <- & -> & pts)".
+      iDestruct "reins" as "[reins _]".
+
+      (* The loaded timestamp is greater or equal to the one we know of. *)
+      assert (store_view TV !!0 ℓ ≤ SV !!0 ℓ).
+      { f_equiv. solve_view_le. }
+      assert (t_i ≤ t_l) as lte by lia.
+
+      (* [σ_l] *)
+      eassert _ as  temp. { eapply (read_atomic_location t_i t_l (OCV !!0 ℓ)); (done || lia). }
+      destruct temp as (σ_l & encσ_l & absHistLook & ? & ? & <- & orderRelated).
+      iDestruct (big_sepM2_delete with "predFullReadHolds") as "[predF predFullReadRest]";
+        [done|done|].
+      simpl.
+      destruct (decide (_)) as [ ?H | contra ].
+      (* we know [t_l] is an exclusive timestamp. *)
+      2: { exfalso. apply contra.
+           split; first lia. rewrite -Nat.add_1_r //. }
+      iDestruct (predicate_holds_phi_decode with "predFullEquiv predF") as "predF";
+        first done.
+
+      (* [σ_p] *)
+      iDestruct "predPersHolds" as (t_p encσ_p msg_p ? ? ?) "[pview predP]".
+      iAssert (⌜ ∃ σ_p, decode encσ_p = Some σ_p ⌝)%I as (σ_p) "%Hdecodeσ_p". {
+        iDestruct "predP" as (pred_pers) "[#eqP _]".
+        iEval (rewrite discrete_fun_equivI) in "predPersEquiv".
+        iSpecialize ("predPersEquiv" $! encσ_p).
+        iEval (rewrite discrete_fun_equivI) in "predPersEquiv".
+        iSpecialize ("predPersEquiv" $! (msg_val msg_p)).
+        iRewrite "predPersEquiv" in "eqP".
+        iPoseProof (encode_predicate_decode (p_pers prot) encσ_p (msg_val msg_p) pred_pers with "eqP") as (σ_p) "%decodeSP".
+        iExists _. done. }
+      iDestruct (predicate_holds_phi_decode with "predPersEquiv predP") as "predP";
+        first done.
+
+      iDestruct ("impl" $! _ _ σ_p (msg_val msg_p)) as "impl".
+      iDestruct ("impl" $! orderRelated) as "[_ [impl _]]".
+      iDestruct ("impl" with "[//]") as "(above & below & P_acc & impl1 & impl2)".
+      rewrite ?monPred_at_objectively.
+      iDestruct ("above" with "[$]") as "%above".
+
+      iAssert 
+        ⌜increasing_map (encode_relation sqsubseteq) (<[(t_l + 1)%nat := encode σ_t]> abs_hist)⌝%I as %incri.
+      {
+        iApply (bi.pure_mono).
+        { apply
+            (increasing_map_insert_succ _ _ _ _ (encode σ_t) increasing
+                                          absHistLook).
+          eapply encode_relation_decode_iff; eauto using decode_encode. }
+        iIntros (t_c encσ_c a ?).
+        assert (OCV !!0 ℓ < t_c) by lia.
+
+        assert (is_Some (phys_hist !! t_c)) as [[v_c cSV cFV ?] look2].
+        { rewrite -elem_of_dom domEq elem_of_dom. done. }
+
+        eassert _ as  temp. { eapply (read_atomic_location_no_inv (t_l) t_c); done || lia. }
+        destruct temp as (s_c & encSC & ? & decodeS' & orderRelated2).
+        simplify_eq.
+        rewrite /encode_relation. rewrite decode_encode. rewrite decodeS'.
+        simpl.
+
+        iSpecialize ("below" $! s_c v_c orderRelated2).
+        iEval (monPred_simpl) in "below".
+        (* we need to justify precondition for the "below" clause,
+         * and we need to distinguish whether [t_c] is the max timestamp.
+         * but first, we extract the full predicate at max timestamp for both cases. *)
+        set t_max := (max_msg phys_hist).
+        assert (t_c ≤ t_max) by (apply max_list_elem_of_le, elem_of_elements, elem_of_dom; done).
+        assert (is_Some (phys_hist !! t_max)) as [[v_max maxSV maxFV ?] look_max]. {
+          apply elem_of_dom.
+          rewrite /max_msg.
+          apply elem_of_elements.
+          apply max_list_elem_of.
+          assert (t_c ∈ dom phys_hist) by (apply elem_of_dom; done).
+          rewrite elements_empty_iff.
+          set_solver.
+        }
+        assert (is_Some (abs_hist !! t_max)) as [e_max look_max'].
+        { rewrite -elem_of_dom -domEq elem_of_dom. done. }
+        eassert _ as  temp. { eapply (read_atomic_location_no_inv t_c t_max); try done || lia. }
+        destruct temp as (s_max & encMax & ? & decodeSMax & orderRelated_max).
+        simplify_eq.
+        iDestruct (big_sepM2_delete with "predFullReadRest") as "[predMax predFullReadRest]".
+        { rewrite lookup_delete_ne; [apply look_max | lia ]. }
+        { rewrite lookup_delete_ne; [apply look_max' | lia]. }
+        simpl.
+        destruct (decide (_)) as [ ?H | contra ].
+        (* we know [t_max] is an exclusive timestamp. *)
+        2: { exfalso. apply contra.
+             split; first lia.
+             rewrite -Nat.add_1_r. apply lookup_max_msg_succ. }
+        iDestruct (predicate_holds_phi_decode with "predFullEquiv predMax") as "predMax";
+          first done.
+        (* we now case analysis whether [t_c] is the final timestamp *)
+        destruct (decide (t_c = t_max)) as [ <- | ].
+        - (* in case [t_c] is max timestamp, we do not need to extract further go with the left branch. *)
+          simplify_map_eq.
+          iApply ("below" $! (TV ⊔ (SV_l, FV_l, ∅) ⊔ (_, _, _)) with "[%] [predF] [predMax]").
+          { rewrite -assoc. apply thread_view_le_l. }
+          2: { iLeft. iApply monPred_mono; last iApply "predMax".
+               apply thread_view_le_r. }
+          { iApply monPred_mono; last iApply "predF".
+            destruct TV as [[??]?].
+            rewrite thread_view_lub.
+            solve_view_le. }
+        - (* in case [t_c] is not max timestamp, we need to extract [p_read] for it and
+           *  go with the right branch. *)
+          iDestruct (big_sepM2_lookup _ _ _ t_c with "predFullReadRest") as "predFR". 
+          { rewrite 2?lookup_delete_ne; [apply look2 | lia | lia ]. }
+          { rewrite 2?lookup_delete_ne; [apply a | lia | lia ]. }
+          simpl.
+          iAssert (p_read prot s_c v_c (cSV, msg_persisted_after_view, ∅))%I
+            with "[predFR]" as "predC".
+          { iApply (predicate_holds_phi_decode with "predReadEquiv"); first done.
+            destruct (decide (_)).
+            - iDestruct ("predFullReadSplit" with "predFR") as "$".
+            - iApply "predFR". }
+          iAssert (((_ ∗ _): dProp Σ) (_ ⊔ _))%I with "[predC predMax]" as "pred". {
+            rewrite monPred_at_sep.
+            iSplitL "predC".
+            { iApply monPred_mono; [ | iAccu ].
+              apply thread_view_le_l. }
+            { iSimpl in "predMax". iApply monPred_mono; [ | iAccu ].
+              apply thread_view_le_r. }
+          }
+          iDestruct (monPred_at_sep with "pred") as "[predC predMax]".
+          iApply ("below" $! (TV ⊔ (SV_l, FV_l, ∅) ⊔ (_, _, _)) with "[%] [predF] [predC predMax]").
+          { rewrite -assoc. apply thread_view_le_l. }
+          2: { iRight.
+               iSplitL "predC".
+               { iApply monPred_mono; last iFrame.
+                 apply thread_view_le_r. }
+               iExists s_max, v_max.
+               iFrame "%".
+               iApply monPred_mono; last iFrame.
+               apply thread_view_le_r. }
+          { iApply monPred_mono; last iApply "predF".
+            destruct TV as [[??]?].
+            rewrite thread_view_lub.
+            solve_view_le. } }
+      set view_l := (SV_l, _, _).
+      set msg_t := (msg in <[t_l + 1 := msg]> _).
+
+      (* we extract the objective fraction from [p_pers] *)
+      iDestruct ("P_acc" with "predP") as "[P P_acc]".
+      rewrite monPred_at_objectively.
+
+      iDestruct ("impl1" $! view_l with "[predF P]") as "[predR R]".
+      { iSplitL "predF"; last done.
+        iApply (monPred_mono with "[$]").
+        solve_view_le. }
+
+      iEval (monPred_simpl) in "impl2".
+      iDestruct ("impl2" $! (view_l ⊔ TV) with "[] [R]") as "> (predF & P & Q)".
+      { iPureIntro. apply thread_view_le_r. }
+      { iApply monPred_mono; last iApply "R". apply thread_view_le_l. }
+
+      (* we recover [P_pers] from the objective fragment *)
+      iEval (rewrite monPred_at_wand) in "P_acc".
+      iEval (rewrite monPred_at_objectively) in "P".
+      iDestruct ("P_acc" with "[//] P") as "predP".
+
+      (* Before we close [interp], we need to obtain the knowledge about [σ_l]
+       * and [msg_l] for [seen_state]. *)
+      iMod (auth_map_map_lookup _ _ _ t_l with "physHists") as "[physHists #know_msg_l]".
+      { done. } { done. }
+      iAssert (know_frag_history_loc ℓ t_l σ_l)%I as "#know_σ_l".
+      { rewrite /know_frag_history_loc /frag_entry_unenc.
+        iExists encσ_l.
+        iPoseProof (big_sepM_lookup _ _ t_l with "frags") as "$"; done. }
+      iMod ("reins" $! (t_l + 1) σ_t
+        with "[%] [//] [//] [] [] physHists [predFullReadRest predR predF] [pview predP] fullHist [//] pts")
+          as "(#frag & #physHistFrag & $)".
+      { lia. }
+      { iPureIntro. simpl. rewrite lookup_zero_insert. lia. }
+      { done. }
+      { (* We insert [predR] first by temporarily hack the internal lookup of [phys_hist] *)
+        iAssert ([∗ map] t ↦ msg;encσ ∈ (delete t_l phys_hist); (delete t_l abs_hist), 
+                   if decide (OCV !!0 ℓ ≤ t ∧ phys_hist !! S t = None ∧ t ≠ t_l)
+                   then
+                     encoded_predicate_holds encp_full encσ (msg_val msg)
+                       (msg_store_view msg, msg_persisted_after_view msg, ∅)
+                   else
+                     encoded_predicate_holds encp_read encσ (msg_val msg)
+                       (msg_store_view msg, msg_persisted_after_view msg, ∅))%I
+          with "[predFullReadRest]" as "predFullReadHolds".
+        { iApply (big_sepM2_impl with "predFullReadRest").
+          iIntros "!>" (t msg encσ look1 look2) "H".
+          assert (t ≠ t_l). {
+            intro eq.
+            simplify_eq.
+            rewrite lookup_delete // in look1. }
+          destruct (decide _); destruct (decide _); naive_solver. }
+        
+        (* We now insert [predR]. *)
+        iPoseProof (big_sepM2_insert_delete _ _ _ _ (Msg _ _ _ _) with "[$predFullReadHolds predR]")
+          as "predFullReadHolds".
+        { destruct (decide _) as [ [_ [_ []]] | ]; first done.
+          iApply (predicate_holds_phi_decode_2 with "predReadEquiv predR"); first done. }
+        
+        (* We now insert the [predF]. *)
+        iPoseProof (big_sepM2_insert _ _ _ (t_l + 1) msg_t with "[$predFullReadHolds predF]")
+          as "predFullReadHolds".
+        { rewrite lookup_insert_ne //. lia. }
+        { rewrite -not_elem_of_dom dom_insert -domEq not_elem_of_union not_elem_of_dom.
+          split; last set_solver.
+          apply not_elem_of_singleton.
+          lia. }
+        { destruct TV as [[? ?] ?].
+          iDestruct (into_no_buffer_at with "predF") as "predF".
+          destruct (decide _).
+          - iApply (predicate_holds_phi with "predFullEquiv"); first reflexivity.
+            iApply (monPred_mono with "predF").
+            subst msg_t.
+            repeat split; last done.
+            * eapply view_lub_le; solve_view_le.
+            * solve_view_le.
+          - iApply (predicate_holds_phi with "predReadEquiv"); first reflexivity.
+            iPoseProof (full_read_split with "predF") as "[predR _]".
+            iApply (monPred_mono with "predR").
+            subst msg_t.
+            repeat split; last done.
+            * eapply view_lub_le; solve_view_le.
+            * solve_view_le. }
+        rewrite (insert_id phys_hist) // (insert_id abs_hist) //.
+        iApply (big_sepM2_impl with "[$]").
+        iIntros (t msg encσ msgLook encSLook) "!> H".
+        destruct (decide (t = t_l)) as [ -> | neq ].
+        - rewrite ?Nat.add_1_r lookup_insert.
+          rewrite ?decide_False; naive_solver.
+        - rewrite lookup_insert_ne; last lia.
+          destruct (decide _); destruct (decide _); naive_solver. }
+      { iExists t_p, encσ_p, msg_p.
+        assert (t_p ≠ t_l + 1).
+        { intro eq.
+          rewrite -> eq in *.
+          simplify_map_eq.
+          (* TODO: make this hypothesis named. *)
+          rewrite H10 // in H4. }
+        rewrite ?lookup_insert_ne //.
+        iFrame "∗".
+        repeat (iSplitPure; first done).
+        by iApply (predicate_holds_phi_decode_2 with "[//] predP"). }
+      iModIntro.
+
+      iSplitPure. { solve_view_le. }
+
+      Opaque mapsto_at seen_state.
+      
+      iSpecialize ("Φpost" $! _ true σ_l).
+      iEval (monPred_simpl) in "Φpost".
+      iApply "Φpost".
+      { iPureIntro. solve_view_le. }
+      iLeft.
+      iSplitPure; first done.
+      iSplitL "Q".
+      { subst view_l.
+        rewrite /post_fence. simpl.
+        iApply monPred_mono; last iApply "Q".
+        repeat destruct_thread_view; repeat destruct_thread_view_le.
+        rewrite thread_view_lub.
+        assert (SV ⊔ SV_l ⊑ <[ℓ:=MaxNat (t_l - (OCV !!0 ℓ) + 1)]> (SV ⊔ SV_l)) as le2.
+        { apply view_insert_le. rewrite lookup_zero_lub. lia. }
+        apply thread_view_le.
+        - etrans; last apply le2. solve_view_le.
+        - apply view_lub_le; solve_view_le.
+        - simpl_view. solve_view_le. }
+      (* [mapsto_at] *)
+      iSplitL.
+      { iExists _, _, _, (t_l + 1). iExistsN.
+        iSplitPure. { rewrite last_snoc. reflexivity. }
+        iSplitPure. { eapply map_sequence_insert_snoc; try done. lia. }
+        iSplitPure.
+        { eapply map_sequence_insert_snoc; last done; first lia.
+          eapply map_no_later_dom; last apply nolater.
+          done. }
+
+        iSplitPure.
+        { eapply map_no_later_insert; last done. lia. }
+        iSplitPure.
+        { rewrite 2!dom_insert_L. rewrite absPhysHistDomEq. done. }
+        simpl.
+        iFrameF "isAtLoc".
+        rewrite big_sepM_insert. 2: { apply nolater. lia. }
+                               rewrite big_sepM_insert.
+        2: {
+          eapply map_dom_eq_lookup_None; first done.
+          apply nolater. lia. }
+        rewrite -know_protocol_unfold.
+        iFrameF "locationProtocol".
+        iSplitPure.
+        { apply: increasing_map_insert_last; try done. lia.
+          etrans; done. }
+        iSplit.
+        (* { iFrame "frag absHist". } *)
+        { simpl. rewrite monPred_at_sep. simpl. iFrame "frag".
+          rewrite -monPred_at_big_sepM.
+          iApply objective_at.
+          rewrite monPred_at_big_sepM.
+          iEval (rewrite monPred_at_big_sepM).
+          simpl.
+          iFrame "absHist". }
+        iFrame "offset".
+        iSplit; last first.
+        { simpl. iPureIntro.
+          rewrite lookup_zero_insert.
+          lia. }
+        simpl.
+
+        iSplit.
+        { simpl. iFrame "physHistFrag". solve_view_le. }
+        rewrite -?monPred_at_big_sepM.
+        iApply monPred_mono; last iApply "physHist".
+        etrans; first apply incl.
+        etrans; first apply incl2.
+        repeat split; solve_view_le. }
+      iExists _, (OCV !!0 ℓ), (Msg v_l SV_l FV_l FV_l).
+      iSplit; last first.
+      { iFrameF "know_msg_l".
+        iPureIntro.
+        simpl.
+        solve_view_le. }
+      iFrameF "locationProtocol".
+      iFrameF "know_σ_l".
+      iFrameF "offset".
+      iPureIntro.
+      simpl.
+      rewrite lookup_zero_insert.
+      lia.
+    - (* failure *)
+      iDestruct "H" as "(-> & -> & pts)".
+      iDestruct "reins" as "[_ reins]".
+      iModIntro.
+
+      (* The loaded timestamp is greater or equal to the one we know of. *)
+      assert (store_view TV !!0 ℓ ≤ SV !!0 ℓ).
+      { f_equiv. solve_view_le. }
+      assert (t_i ≤ t_l) as lte by lia.
+
+      eassert _ as  temp. { eapply (read_atomic_location t_i t_l (OCV !!0 ℓ)); (done || lia). }
+      destruct temp as (σ_l & encσ_l & ? & ? & ? & <- & orderRelated).
+
+      iDestruct (big_sepM2_lookup_acc with "predFullReadHolds") as "[predFR predFullReadHolds]";
+        [done|done|].
+      simpl.
+      destruct (decide (_)) as [ ?H | contra ].
+      (* we know [t_l] is an exclusive timestamp. *)
+      2: { exfalso. apply contra.
+           split; first lia. rewrite -Nat.add_1_r //. }
+      
+      iDestruct (predicate_holds_phi_decode with "predFullEquiv predFR") as "predF";
+        first done.
+
+      iDestruct ("impl" $! _ _ _ _ orderRelated) as "[_ [_ [impl Q3]]]".
+      iEval (rewrite monPred_at_objectively) in "impl".
+      iSpecialize ("impl" $! (∅, ∅, ∅)).
+      iEval (monPred_simpl) in "impl".
+      iDestruct ("impl" $! _ with "[%] predF") as "[predF Q2]"; first solve_view_le.
+      
+      iSpecialize ("predFullReadHolds" with "[predF]").
+      { iApply predicate_holds_phi_decode; done. }
+
+      iDestruct ("reins" with "[$] [$] [$] [$] [$]") as "$".
+
+      iSplitPure. { repeat split; try done; apply view_le_l. }
+
+      iSpecialize ("Φpost" $! _ false σ_l).
+      iEval (monPred_simpl) in "Φpost".
+      iApply "Φpost".
+
+      { iPureIntro.
+        etrans; first done.
+        repeat split; auto using view_le_l. }
+      iRight.
+      iSplitPure; first done.
+      iSplitPure; first done.
+      rewrite /post_fence. simpl.
+      iSplit.
+      { (* We show what is, essentially, the points-to predicate that we started with. *)
+        iExistsN.
+        iFrameF (lastEq).
+        iFrameF (slice).
+        iFrameF (slicePhys).
+        iFrameF (nolater).
+        iFrameF (absPhysHistDomEq).
+        iFrameF "isAtLoc".
+        iFrameF "locationProtocol".
+        iSplitPure; first done.
+        iSplit.
+        { iApply objective_at.
+          iEval (rewrite monPred_at_big_sepM).
+          iFrame "absHist". }
+        iSplit.
+        { iEval (rewrite -monPred_at_big_sepM) in "physHist".
+          iApply monPred_mono; last iApply "physHist".
+          etrans; first apply incl.
+          etrans; first apply incl2.
+          solve_view_le. }
+        iFrameF "offset".
+        iPureIntro.
+        etrans; first apply tSLe.
+        simpl.
+        f_equiv.
+        solve_view_le. }
+      iSplitL "Q2"; iApply monPred_mono; try iFrame.
+      { repeat split; eauto using view_le_r, view_empty_least.
+        rewrite assoc. apply view_le_r. }
+      { etrans; first done. etrans; first done. repeat split; auto using view_le_l. }
+      (* these shelved goals seem to be [s_p] and [v_p] for the safe comparison and failure case
+       * it's probably better to rewrite the quantifiers, but not an important problem *)
+      Unshelve. all: done.
+  Qed.
+
+    (* (** [Q1] is the resource we want to extract in case of success and and [Q2] is *)
+  (* the resource we want to extract in case of failure. *) *)
+  (* Lemma wp_cas_at Q1 Q2 Q3 ℓ prot `{!ProtocolConditions prot} ss s_i *)
+  (*     (v_i v_t : val) R s_t st E : *)
+  (*   {{{ *)
+  (*     ℓ ↦_AT^{prot} (ss ++ [s_i]) ∗ *)
+  (*     (∀ s_l v_l, ⌜ s_i ⊑ s_l ⌝ -∗ *)
+  (*       ((▷ prot.(p_inv) s_l v_l) -∗ ⌜ vals_compare_safe v_i v_l ⌝) ∗ *)
+  (*       (((* in case of success *) *)
+  (*         (* The state we write fits in the history. *) *)
+  (*         ⌜ s_l ⊑ s_t ⌝ ∗ *)
+  (*         (∀ s_n v_n, ⌜ s_l ⊑ s_n ⌝ -∗ prot.(p_inv) s_l v_l -∗ *)
+  (*           prot.(p_inv) s_n v_n -∗ ⌜ s_t ⊑ s_n ⌝) ∗ *)
+  (*         (* Extract from the location we load. *) *)
+  (*         (<obj> (prot.(p_inv) s_l v_l -∗ prot.(p_inv) s_l v_l ∗ R s_l)) ∗ *)
+  (*         (* Establish the invariant for the value we store. *) *)
+  (*         (R s_l -∗ prot.(p_inv) s_t v_t ∗ Q1 s_l)) *)
+  (*       ∧ (* in case of failure *) *)
+  (*         ((<obj> (prot.(p_inv) s_l v_l -∗ prot.(p_inv) s_l v_l ∗ Q2 s_l)) ∗ Q3) *)
+  (*       )) *)
+  (*   }}} *)
+  (*     CAS #ℓ v_i v_t @ st; E *)
+  (*   {{{ b s_l, RET #b; *)
+  (*     (⌜ b = true ⌝ ∗ <fence> Q1 s_l ∗ ℓ ↦_AT^{prot} ((ss ++ [s_i]) ++ [s_t])) ∨ *)
+  (*     (⌜ b = false ⌝ ∗ ⌜ s_i ⊑ s_l ⌝ ∗ ℓ ↦_AT^{prot} (ss ++ [s_i]) ∗ <fence> (Q2 s_l) ∗ Q3) *)
+  (*   }}}. *)
+  (* Proof. *)
+  (*   intros Φ. *)
+  (*   iIntros "H Φpost". *)
+  (*   iApply (wp_bind ([SndCtx])). *)
+  (*   iApply (wp_cmpxchg_at with "H"). *)
+  (*   iIntros "!>" (v b s_l) "disj /=". *)
+  (*   iApply wp_pure_step_later; first done. *)
+  (*   iNext. *)
+  (*   iApply wp_value. *)
+  (*   iApply "Φpost". *)
+  (*   iApply "disj". *)
+  (* Qed. *)
+End wp_at.
