src/high/weakestpre/at/load.v
@@ -1,0 +1,721 @@
+From iris.proofmode Require Import proofmode monpred.
+From iris.algebra Require Import gset.
+From iris_named_props Require Import named_props.
+
+From self Require Import extra solve_view_le encode_relation map_extra view_slice.
+
+From self.lang Require Import syntax tactics lemmas.
+
+From self.base Require Import generational_resources primitive_laws.
+
+From self.high Require Import wrappers monpred_simpl protocol locations crash_weakestpre weakestpre.
+From self.high.modalities Require Import post_fence_sync_advanced.
+From self.high.lib Require Import abstract_state increasing_map.
+From self.high.weakestpre.at Require Import prelude.
+
+From self Require Export lang.
+From self.high Require Export dprop.
+
+Set Default Proof Using "Type*".
+
+Section wp_at.
+  Context `{AbstractState ST}.
+  Context `{!nvmBaseGS Σ Ω, !nvmHighGS Σ Ω, PerennialG Σ}.
+
+  Implicit Types (ℓ : loc) (σ : ST) (prot : LocationProtocol ST).
+
+  Lemma map_sequence_big_sepM_sepL {A} (m : gmap nat A) lo hi ss (ϕ : A  → iProp Σ) :
+    map_sequence m lo hi ss →
+    ([∗ map] k ↦ y ∈ m, ϕ y) -∗
+    ([∗ list] y ∈ ss, ϕ y) ∗ (([∗ list] y ∈ ss, ϕ y) -∗ [∗ map] k ↦ y ∈ m, ϕ y).
+  Proof.
+    generalize dependent m.
+    generalize dependent lo.
+    induction ss as [|x ss' IH]; first done.
+    iIntros (lo m seq) "M".
+    destruct ss' as [|x2 ss''].
+    { destruct seq as [look ->]. rewrite /= right_id.
+      iApply (big_sepM_lookup_acc with "M"). done. }
+    simpl.
+    destruct seq as (look & lo2 & ? & ? & ?).
+    iDestruct (big_sepM_delete with "M") as "[$ M]"; first done.
+    iDestruct (IH lo2 with "M") as "[horse bing]".
+    { apply map_sequence_delete_below; done. }
+    simpl.
+    iFrame "horse".
+    iIntros "[Hx Hx2]".
+    iDestruct ("bing" with "Hx2") as "H2".
+    iApply big_sepM_delete; first done.
+    iFrame.
+  Qed.
+
+  Lemma map_sequence_big_sepM2_sepL2 {A B}
+    (m1 : gmap nat A) (m2 : gmap nat B) tLo tHi ss ms
+    (ϕ : A  → B → iProp Σ) :
+    map_sequence m1 tLo tHi ss →
+    map_sequence m2 tLo tHi ms →
+    ([∗ map] k ↦ y1;y2 ∈ m1;m2, ϕ y1 y2) -∗
+    ([∗ list] y1;y2 ∈ ss;ms, ϕ y1 y2) ∗
+    (([∗ list] y1;y2 ∈ ss;ms, ϕ y1 y2) -∗ [∗ map] k ↦ y1;y2 ∈ m1;m2, ϕ y1 y2).
+  Proof.
+    iIntros (seq1 seq2).
+    rewrite big_sepM2_alt.
+    rewrite big_sepL2_alt.
+    iIntros "(%domEq & M)".
+    assert (length ss = length ms) as lenEq.
+    { eapply map_sequence_dom_length; done. }
+    iFrame (lenEq).
+    iDestruct (map_sequence_big_sepM_sepL with "M") as "[L Lreins]".
+    { apply map_sequence_zip; done. }
+    iFrame "L".
+    iIntros "[_ L]".
+    iDestruct ("Lreins" with "L") as "$".
+    iPureIntro. done.
+  Qed.
+
+  (* Lemma bingo {A B} (m1 : gmap nat A) (m2 : gmap nat B) tLo tHi ss ms *)
+  (*   (ϕ : A  → B → dProp Σ) : *)
+  (*   map_sequence m1 tLo tHi ss → *)
+  (*   map_sequence m2 tLo tHi ms → *)
+  (*   ⊢ ([∗ list] y1;y2 ∈ ss;ms, ϕ y1 y2) ∗-∗ ([∗ map] k ↦ y1;y2 ∈ m1;m2, ϕ y1 y2). *)
+  (* Proof. *)
+  (*   iIntros (seq1 seq2). *)
+  (* Qed. *)
+
+  (* Lemma big_sepM2_union {A B} (Φ : nat → A → B → iProp Σ) (m1 m2 : gmap nat A) *)
+  (*     (n1 n2 : gmap nat B) : *)
+  (*   m1 ##ₘ m2 → *)
+  (*   n1 ##ₘ n2 → *)
+  (*   ([∗ map] k↦y1;y2 ∈ (m1 ∪ m2);(n1 ∪ n2), Φ k y1 y2) *)
+  (*   ⊣⊢ ([∗ map] k↦y1;y2 ∈ m1;n1, Φ k y1 y2) ∗ ([∗ map] k↦y1;y2 ∈ m2;n2, Φ k y1 y2). *)
+  (* Proof. *)
+  (*   intros disj1 disj2. *)
+  (*   rewrite !big_sepM2_alt. *)
+  (*   rewrite big_sepM_union. *)
+  (*   apply big_opM_union. *)
+  (* Qed. *)
+
+  (* Lemma bingobongo (ϕ : ST → _) (pred : enc_predicateO) physHist absHist *)
+  (*     encAbsHist fullEncAbsHist : *)
+  (*   absHist = omap decode encAbsHist → *)
+  (*   encAbsHist ⊆ fullEncAbsHist → *)
+  (*   (pred ≡ encode_predicate ϕ) -∗ *)
+  (*   encoded_predicate_hold physHist fullEncAbsHist pred -∗ *)
+  (*   ([∗ map] msg;s ∈ physHist;absHist, *)
+  (*     ϕ s (msg_val msg) _ (msg_store_view msg, msg_persisted_after_view msg, ∅)). *)
+
+  Definition fold_views (m : history) :=
+    map_fold
+      (λ _ msg (TV : thread_view),
+        (msg_store_view msg, msg_persisted_after_view msg, ∅) ⊔ TV) (∅, ∅, ∅) m.
+
+  Lemma fold_views_in_phys_hist phys_hist t msg :
+    phys_hist !! t = Some msg →
+    (msg_store_view msg, msg_persisted_after_view msg, ∅) ⊑ fold_views phys_hist.
+  Proof.
+    rewrite /fold_views. simpl.
+    apply (map_fold_ind (λ res phys_hist, phys_hist !! t = Some msg → _ ⊑ res)).
+    - inversion 1.
+    - intros t2 ???? IH.
+      destruct (decide (t = t2)) as [->|ne].
+      * rewrite lookup_insert.
+        inversion 1.
+        apply thread_view_le_l.
+      * rewrite lookup_insert_ne; last done.
+        rewrite -thread_view_le_r.
+        apply IH.
+  Qed.
+
+  (* This lemma extracts a list of predicates held over all existing
+   * timestamps. This is only true for [read] predicates in the new model.
+   * *)
+  Lemma extract_list_of_preds abs_hist (phys_hist : history) tLo tS ss ms prot ℓ encAbsHist (predRead : enc_predicateO) :
+    abs_hist = omap decode encAbsHist →
+    map_sequence abs_hist tLo tS ss →
+    map_sequence phys_hist tLo tS ms →
+    dom abs_hist = dom phys_hist →
+    predRead ≡ encode_predicate (p_read prot) -∗
+    ([∗ map] t↦msg;encS ∈ phys_hist; encAbsHist, encoded_predicate_holds predRead encS
+                                                   (msg_val msg)
+                                                   (msg_store_view msg,
+                                                    msg_persisted_after_view msg, ∅)) -∗
+    ([∗ list] s;v ∈ ss;(msg_val <$> ms), p_read prot s v) (fold_views phys_hist).
+  Proof.
+    iIntros (-> seqAbs seqPhys domEq) "#equiv P".
+    iDestruct (big_sepM2_impl_dom_subseteq _ _ _ _ phys_hist (omap decode encAbsHist) with "P []") as "P".
+    { done. }
+    { done. }
+    { iIntros "!>" (t m es m2 s ? encLook ? look) "H".
+      apply lookup_omap_Some in look as (? & ? & ?).
+      assert (m = m2) as <- by congruence.
+      assert (es = x) as <- by congruence.
+      iDestruct (predicate_holds_phi_decode_1 with "equiv H") as "H"; first done.
+      iApply "H". }
+    iDestruct (map_sequence_big_sepM2_sepL2 with "P") as "[P Lreins]"; first done.
+    { done. }
+    rewrite big_sepL2_flip.
+    rewrite monPred_at_big_sepL2.
+    rewrite big_sepL2_fmap_r.
+    iApply (big_sepL2_impl with "P").
+    iIntros "!>" (idx s msg ? msLook) "pred".
+    iApply monPred_mono; last iApply "pred".
+    eapply map_sequence_list_lookup in msLook as (? & ? & look); last apply seqPhys.
+    eapply fold_views_in_phys_hist.
+    done.
+  Qed.
+
+  Lemma wp_load_at ℓ ss s Q1 Q2 prot `{!ProtocolConditions prot} st E :
+    {{{
+      ℓ ↦_AT^{prot} (ss ++ [s]) ∗
+      (* The case where we read an already known write. *)
+      ((∀ vs vL, ∃ P (_ : Objective P) (_ : Persistent P),
+        ⌜ last vs = Some vL ⌝ -∗
+        (* Extract knowledge from all the predicates. *)
+        (([∗ list] s; v ∈ ss ++ [s];vs, prot.(p_read) s v) -∗ P) ∗
+        (* Using the [P] and the predicate for the loaded location show [Q1]. *)
+        (P -∗ <obj> (prot.(p_read) s vL -∗ Q1 vL ∗ prot.(p_read) s vL))) ∧
+      (* The case where we read a new write. *)
+      (∀ vs vL sL, ∃ P (_ : Objective P) (_ : Persistent P),
+        ⌜ s ⊑ sL ⌝ -∗
+        (* Extract knowledge from all the predicates. *)
+        (([∗ list] s; v ∈ (ss ++ [s]) ++ [sL];vs ++ [vL], prot.(p_read) s v) -∗ P) ∗
+        (P -∗ <obj> (prot.(p_read) sL vL -∗ Q2 sL vL ∗ prot.(p_read) sL vL))))
+    }}}
+      !_AT #ℓ @ st; E
+    {{{ vL, RET vL;
+      (∃ sL, ℓ ↦_AT^{prot} ((ss ++ [s]) ++ [sL]) ∗ <fence> Q2 sL vL) ∨
+      (* We didn't have to give the points-to predicate back here, but doing
+       * that is useful for users of the lemma. *)
+      (ℓ ↦_AT^{prot} (ss ++ [s]) ∗ <fence> Q1 vL)
+    }}}.
+  Proof.
+    intros Φ.
+    iModel.
+    iDestruct 1 as "(#pts & pToQ)".
+    iAssert (_) as "ptsCopy". { iApply "pts". }
+    iDestruct "pts" as (abs_hist phys_hist tLo tS offset s' ms) "H". iNamed "H".
+    assert (s' = s) as ->. { apply (inj Some). rewrite -lastEq. apply last_snoc. }
+    iDestruct "tSLe" as %tSLe.
+    (* iDestruct (store_lb_protocol with "storeLb") as "#knowProt". *)
+    iNamed "locationProtocol".
+    (* rewrite /store_lb. *)
+    (* iDestruct "storeLb" as (tS offset) "(#prot & #hist & #offset & %tSLe)". *)
+
+    (* We unfold the WP. *)
+    iIntros (TV' incl) "Φpost".
+    iApply wp_unfold_at.
+    iIntros ([[SV PV] BV] incl2) "#val".
+
+    iApply wp_extra_state_interp. { done. } { by apply prim_step_load_acq_no_fork. }
+
+    (* We open [interp]. *)
+    iIntros "interp".
+    iAssert (∃ OCV, crashed_at_offset OCV ∗ ⌜ OCV !!0 ℓ = offset ⌝)%I as (OCV) "[#offsets <-]".
+    { iDestruct "offset" as (?) "(? & ? & %)".
+      iExists _.
+      by iFrame "#". }
+    simpl.
+    iDestruct (interp_get_at_loc with "interp isAtLoc [] offset")
+      as (phys_hists phys_hist' abs_hist' encp_full encp_read encp_pers pview) "(R & reins)".
+    { rewrite /know_protocol. iFrameNamed. }
+
+    iNamed "R".
+    iEval (rewrite monPred_at_big_sepM) in "physHist".
+    iEval (rewrite monPred_at_big_sepM) in "absHist".
+    iEval (setoid_rewrite monPred_at_sep) in "physHist".
+    simpl.
+    setoid_rewrite monPred_at_embed.
+
+    iAssert (⌜ phys_hist ⊆ phys_hist' ⌝)%I as %sub.
+    { rewrite map_subseteq_spec.
+      iIntros (?? physHistLook).
+
+      iDestruct (big_sepM_lookup with "physHist") as "[hi frag]"; first done.
+      iDestruct (auth_map_map_auth_frag with "physHists frag") as %(phys_hist'' & ? & ?).
+      assert (phys_hist' = phys_hist'') as <-.
+      { apply (inj Some). rewrite -physHistsLook. done. }
+      done. }
+
+    iDestruct (history_full_entry_frag_lookup_big with "fullHist absHist")
+      as %(encAbsHist & subset & domEq2 & eqeq & map).
+
+    (* We add this to prevent Coq from trying to use [highExtraStateInterp]. *)
+    set (extra := (Build_extraStateInterp _ _)).
+    iApply (@program_logic.crash_weakestpre.wpc_wp).
+    iApply @wpc_fupd.
+    iApply @program_logic.crash_weakestpre.wp_wpc.
+
+    iApply (wp_load_acquire_alt (extra := {| extra_state_interp := True |})
+             with "[$offsets $pts $val]").
+    iIntros "!>" (tL vL SV' PV' _PV') "(%look & %gt & #val' & pts)".
+
+    iFrame "val'".
+
+    assert (store_view TV !!0 ℓ ≤ SV !!0 ℓ).
+    { f_equiv. solve_view_le. }
+    assert (tS ≤ tL) as lte by lia.
+    
+    assert (abs_hist !! tS = Some s).
+    { rewrite -lastEq. eapply map_sequence_lookup_hi; done. }
+    iDestruct (big_sepM_lookup with "absHist") as "hist"; first done.
+    iDestruct (history_full_entry_frag_lookup with "fullHist hist")
+      as %(enc & lookTS & decodeEnc).
+
+    rewrite <- pure_sep_l; last solve_view_le.
+
+    (* The final view under the post fence modality where we will have to show
+     * [Q]. *)
+    set (TVfinal := (SV ⊔ SV', PV ⊔ (BV ⊔ PV'), BV ⊔ PV')).
+    assert (TV ⊑ TVfinal).
+    { etrans; first apply incl. etrans; first apply incl2.
+      rewrite /TVfinal.
+      solve_view_le. }
+
+    (*
+    (* All the messages in the physical history are included in [TVfinal]. *)
+    iAssert (
+      ⌜ map_Forall
+        (λ (_ : nat) (msg : message),
+           msg_store_view msg ⊑ store_view TVfinal
+           ∧ msg_persisted_after_view msg ⊑ flush_view TVfinal) phys_hist ⌝
+    )%I as %inTVFinal.
+    { iIntros (? msg looki).
+      iDestruct (big_sepM_lookup with "physHist") as "[[%have %have2] _]"; first done.
+      iPureIntro.
+      split.
+      - solve_view_le.
+      - etrans; first apply have2. rewrite /TVfinal.
+        simpl.
+        destruct TV as [[??]?].
+        destruct TV' as [[??]?].
+        simpl.
+        apply view_lub_le.
+        * solve_view_le.
+        * solve_view_le. }
+    *)
+
+    destruct (decide (tS = tL)) as [eq|neq].
+    - iDestruct "pToQ" as "[pToQ _]".
+      subst.
+
+      assert (last (msg_val <$> ms) = Some vL).
+      { rewrite fmap_last.
+        apply map_sequence_lookup_hi_alt in slicePhys
+          as (msg & physHistLook & ->).
+        eapply map_subseteq_spec in sub; last done.
+        rewrite -sub. rewrite look. done. }
+
+      iDestruct ("pToQ" $! (msg_val <$> ms) vL) as (P ? ?) "pToQ".
+      iDestruct ("pToQ" with "[]") as "[getP getQ]".
+      { iPureIntro. done. }
+
+      iEval (monPred_simpl) in "getP".
+      iDestruct ("getP" $! (TV ⊔ _) with "[%] [-]") as "#P".
+      { apply thread_view_le_l. }
+      { (* Here's the reason we are not merging the two predicates in the lemma:
+         * [phys_hist] is the history known to local thread,
+         * [physHist] is the complete history obtained from [interp].
+         * whether we get [predFull] or [predRead] depends on [physHist],
+         * but the list of holding predicates we want to obtain is from [phys_hist]
+         * which means the [extract_list_of_preds] lemma would
+         * otherwise need to take both of them to work *)
+        iDestruct (extract_list_of_preds
+          with "predReadEquiv [predFullReadHolds]") as "L"; try done.
+        - iPoseProof (big_sepM2_impl_subseteq with "predFullReadHolds") as "P"; try done.
+          { rewrite -domEq2.
+            rewrite absPhysHistDomEq.
+            done. }
+          { iApply (big_sepM2_impl with "P").
+            iIntros "!> %t %msg %encS %physHistLook %absHistLook predFR".
+            destruct (decide (OCV !!0 ℓ ≤ t ∧ phys_hist' !! S t = None)) as [ [] | no ].
+            { assert (is_Some (@decode ST _ _ encS)) as [? ?]. {
+                replace (decode encS) with (encAbsHist !! t ≫= @decode ST _ _) by by rewrite absHistLook.
+                rewrite -lookup_omap.
+                rewrite -elem_of_dom.
+                rewrite domEq2.
+                by rewrite elem_of_dom.
+              }
+              iPoseProof (predicate_holds_phi_decode_1 with "predFullEquiv predFR") as "H"; first done.
+              iPoseProof (full_read_split with "H") as "[Hread _]".
+              iApply (predicate_holds_phi_decode_2 with "predReadEquiv Hread"); first done.
+            }
+            { iApply "predFR". } }
+        - iApply monPred_mono; last done.
+          apply thread_view_le_r. }
+      iEval (monPred_simpl) in "getQ".
+      iDestruct ("getQ" with "[%] [P]") as "bing"; first done.
+      { iApply objective_at. iApply "P". }
+      rewrite monPred_at_objectively.
+
+      eassert _ as temp.
+      { eapply map_Forall_lookup_1; first apply atInvs.
+        replace tL with (tL - (OCV !!0 ℓ) + (OCV !!0 ℓ)) in look by lia.
+        rewrite drop_prefix_lookup. done. }
+      simpl.
+      destruct temp as (? & pvEq).
+      simpl in pvEq.
+
+      iAssert (at_encoded_full_read_predicates_hold abs_hist' phys_hist' (OCV !!0 ℓ) encp_full encp_read ∗
+               Q1 vL (SV', _PV', ∅))%I with "[predFullReadHolds bing]"
+        as "[predFullReadHolds Q]". {
+        (* we now attempt to obtain [p_read] at [tL +  offset]. *)
+        (* again, we need to case distinction over whether it's held at full or read. *)
+        iDestruct (big_sepM2_lookup_acc with "predFullReadHolds") as "[predFR predMap]".
+        { done. } { done. }
+        simpl.
+        destruct (decide _) as [[] | no ].
+        - iDestruct (predicate_holds_phi_decode with "predFullEquiv predFR") as "PH";
+            first done.
+
+          iPoseProof (full_read_split with "PH") as "[PH Prestore]".
+
+          iDestruct ("bing" $! _ with "PH") as "[Q predHolds]".
+
+          iSpecialize ("Prestore" with "predHolds").
+
+          iDestruct ("predMap" with "[Prestore]") as "predMap".
+          { iIntros.
+            iApply (predicate_holds_phi_decode with "predFullEquiv Prestore").
+            assumption. }
+          iFrame.
+        - iDestruct (predicate_holds_phi_decode with "predReadEquiv predFR") as "PH";
+            first done.
+
+          iDestruct ("bing" $! _ with "PH") as "[Q predHolds]".
+
+          iDestruct ("predMap" with "[predHolds]") as "predMap".
+          { iIntros.
+            iApply (predicate_holds_phi_decode with "predReadEquiv predHolds").
+            assumption. }
+          iFrame. }
+      iModIntro.
+
+      (* We re-establish [interp]. *)
+      iDestruct ("reins" with "[$] [$] [$] [$] [$]") as "$".
+
+      iSpecialize ("Φpost" $! vL).
+      monPred_simpl.
+      iApply "Φpost".
+      { iPureIntro.
+        etrans. eassumption.
+        repeat split; try done; try apply view_le_l. }
+      (* The thread view we started with [TV] is smaller than the view we ended
+       * with. *)
+      (* assert (TV ⊑ (SV ⊔ SV', PV, BV ⊔ PV')).
+           { clear H4. do 2 (etrans; first done). repeat split; auto using view_le_l. }
+       *)
+      iRight. simpl.
+      iSplit. {
+        (* We show what is, essentially, the points-to predicate that we started with. *)
+        iExistsN.
+        iFrameF (lastEq).
+        iFrameF (slice).
+        iFrameF (slicePhys).
+        iFrameF (nolater).
+        iFrameF (absPhysHistDomEq).
+        iFrameF "isAtLoc".
+        iFrameNamedF.
+        { iAssumption. }
+        iEval (rewrite monPred_at_big_sepM).
+        setoid_rewrite monPred_at_embed.
+        iFrameF "absHist".
+        iSplit.
+        { iApply (monPred_mono _ (TV)).
+          { etrans; first apply incl.
+            etrans; first apply incl2.
+            solve_view_le. }
+          rewrite monPred_at_big_sepM.
+          setoid_rewrite monPred_at_sep.
+          simpl.
+          setoid_rewrite monPred_at_embed.
+          iApply "physHist". }
+        iFrameF "offset".
+        iPureIntro.
+        etrans; first apply tSLe.
+        f_equiv.
+        solve_view_le. }
+      iApply monPred_mono; last iFrame "Q".
+      rewrite -pvEq.
+      solve_view_le.
+    - iDestruct "pToQ" as "[_ pToQ]".
+
+      iMod (auth_map_map_lookup with "physHists") as "[physHists #physHistFrag]".
+      { done. } { done. }
+
+      eassert _ as temp. { eapply (read_atomic_location tS tL (OCV !!0 ℓ)); (done || lia). }
+      destruct temp as (sL & encSL & ? & ? & ? & <- & orderRelated).
+
+      iDestruct ("pToQ" $! (msg_val <$> ms) vL sL) as (P ? ?) "pToQ".
+      iDestruct ("pToQ" with "[//]") as "[getP getQ]".
+      iEval (monPred_simpl) in "getP".
+      iDestruct ("getP" $! (TVfinal ⊔ _) with "[%] [-]") as "#P".
+      { etrans; first done. apply thread_view_le_l. }
+      { iDestruct (big_sepM2_delete with "predFullReadHolds") as "[phiI predHolds]".
+        { apply look. } { done. }
+        simpl.
+        rewrite big_sepL2_snoc.
+        iSplitR "phiI".
+        - iDestruct (extract_list_of_preds
+                       (delete tL abs_hist)
+                       (delete tL phys_hist)
+                       tLo tS
+          with "predReadEquiv [predHolds]") as "L"; try done.
+          (* iDestruct (extract_list_of_preds _ *)
+          (*   (delete (tL + offset) abs_hist) *)
+          (*   (delete (tL + offset) phys_hist) tLo tS _ _ _ _ _ _ *)
+          (*   with "predEquiv [predHolds]") as "L". *)
+          * rewrite -eqeq. rewrite -omap_delete. reflexivity.
+          * rewrite -eqeq.
+            apply map_sequence_delete_above; first lia.
+            rewrite eqeq.
+            done.
+          * apply map_sequence_delete_above; [lia|done].
+          * rewrite 2!dom_delete_L.
+            rewrite absPhysHistDomEq.
+            set_solver+.
+          * iPoseProof (big_sepM2_impl_subseteq with "predHolds") as "predHolds".
+            + apply delete_mono. done.
+            + apply delete_mono. done.
+            + rewrite 2!dom_delete_L.
+              rewrite -absPhysHistDomEq.
+              rewrite -domEq2.
+              done.
+            + iApply (big_sepM2_impl with "predHolds").
+              iIntros (t msg encS physHistLook absHistLook) "!> predFR".
+              destruct (decide _) as [ [] | no ].
+              { assert (is_Some (@decode ST _ _ encS)) as [? ?]. {
+                  replace (decode encS) with ((delete tL encAbsHist) !! t ≫= @decode ST _ _) by by rewrite absHistLook.
+                  rewrite -lookup_omap.
+                  rewrite -elem_of_dom.
+                  rewrite omap_delete.
+                  rewrite dom_delete.
+                  rewrite eqeq.
+                  rewrite elem_of_difference.
+                  rewrite domEq2.
+                  rewrite elem_of_dom.
+                  apply lookup_delete_Some in absHistLook as [].
+                  set_solver.
+                }
+                iPoseProof (predicate_holds_phi_decode_1 with "predFullEquiv predFR") as "H"; first done.
+                iPoseProof (full_read_split with "H") as "[Hread _]".
+                iApply (predicate_holds_phi_decode_2 with "predReadEquiv Hread"); first done.
+              }
+              { iApply "predFR". }
+          * iApply monPred_mono; last done.
+            apply thread_view_le_r.
+        - destruct (decide _).
+          * iDestruct (predicate_holds_phi_decode with "predFullEquiv phiI") as "phiI";
+              first done.
+            iPoseProof (full_read_split with "phiI") as "[phiI _]".
+            iApply monPred_mono; last iApply "phiI".
+            rewrite /TVfinal.
+            etrans; last apply thread_view_le_l.
+            solve_view_le.
+          * iDestruct (predicate_holds_phi_decode with "predReadEquiv phiI") as "phiI";
+              first done.
+            iApply monPred_mono; last iApply "phiI".
+            rewrite /TVfinal.
+            etrans; last apply thread_view_le_l.
+            solve_view_le. }
+      iEval (monPred_simpl) in "getQ".
+      iDestruct ("getQ" with "[%] [P]") as "bing".
+      { done. }
+      { iApply objective_at. iApply "P". }
+      rewrite monPred_at_objectively.
+
+      eassert _ as temp.
+      { eapply map_Forall_lookup_1; first apply atInvs.
+        replace tL with (tL - (OCV !!0 ℓ) + (OCV !!0 ℓ)) in look by lia.
+        rewrite drop_prefix_lookup. done. }
+      destruct temp as (? & pvEq).
+      simpl in pvEq.
+
+      iAssert (at_encoded_full_read_predicates_hold abs_hist' phys_hist' (OCV !!0 ℓ) encp_full encp_read ∗
+               Q2 sL vL (SV', PV', ∅))%I with "[predFullReadHolds bing]"
+        as "[predFullReadHolds Q]". {
+        (* we now attempt to obtain [p_read] at [tL +  offset].
+         * again, we need to case distinction over whether it's held at full or read. *)
+        iDestruct (big_sepM2_lookup_acc with "predFullReadHolds") as "[predFR predMap]".
+        { done. } { done. }
+        simpl.
+        destruct (decide _) as [[] | no ].
+        - iDestruct (predicate_holds_phi_decode with "predFullEquiv predFR") as "PH";
+            first done.
+
+          iPoseProof (full_read_split with "PH") as "[PH Prestore]".
+
+          iDestruct ("bing" $! _ with "PH") as "[Q predHolds]".
+
+          iSpecialize ("Prestore" with "predHolds").
+
+          iDestruct ("predMap" with "[Prestore]") as "predMap".
+          { iIntros.
+            iApply (predicate_holds_phi_decode with "predFullEquiv Prestore").
+            assumption. }
+          iFrame.
+        - iDestruct (predicate_holds_phi_decode with "predReadEquiv predFR") as "PH";
+            first done.
+
+          iDestruct ("bing" $! _ with "PH") as "[Q predHolds]".
+
+          iDestruct ("predMap" with "[predHolds]") as "predMap".
+          { iIntros.
+            iApply (predicate_holds_phi_decode with "predReadEquiv predHolds").
+            assumption. }
+          iFrame. }
+      iModIntro.
+
+      (* We re-establish [interp]. *)
+      iDestruct ("reins" with "[$] [$] [$] [$] [$]") as "$".
+
+      iSpecialize ("Φpost" $! vL).
+      monPred_simpl.
+      iApply "Φpost".
+      { iPureIntro.
+        etrans. eassumption.
+        repeat split; try done; try apply view_le_l. }
+      iLeft. iExists (sL).
+      iSplitR "Q"; last first.
+      { simpl. iApply monPred_mono; last iFrame "Q".
+        solve_view_le. }
+      iExists (<[ tL := sL ]>abs_hist). iExistsN.
+      iSplitPure. { rewrite last_snoc. reflexivity. }
+      iSplitPure. { eapply map_sequence_insert_snoc; try done. lia. }
+      iSplitPure.
+      { eapply map_sequence_insert_snoc; last done; first lia.
+        eapply map_no_later_dom; last apply nolater.
+        done. }
+      iSplitPure.
+      { eapply map_no_later_insert; last done. lia. }
+      iSplitPure.
+      { rewrite 2!dom_insert_L. rewrite absPhysHistDomEq. done. }
+      iFrameF "isAtLoc".
+      rewrite big_sepM_insert. 2: { apply nolater. lia. }
+      rewrite big_sepM_insert.
+      2: {
+        eapply map_dom_eq_lookup_None; first done.
+        apply nolater. lia. }
+      iFrameNamedF.
+      { iAssumption. }
+      iSplitPure.
+      { apply: increasing_map_insert_last; try done. lia. }
+      rewrite monPred_at_sep.
+      rewrite monPred_at_big_sepM.
+      setoid_rewrite monPred_at_embed.
+      iFrame "absHist".
+      iSplit.
+      { iExists _.
+        iSplitPure; first done.
+        iApply (big_sepM_lookup with "frags"). done. }
+      iFrame "offset".
+      iSplit; last first.
+      { simpl. iPureIntro.
+        rewrite lookup_zero_lub.
+        lia. }
+      simpl.
+      iSplit.
+      { iFrame "physHistFrag".
+        iPureIntro.
+        simpl.
+        solve_view_le. }
+      iApply (monPred_mono _ TV).
+      { etrans; first apply incl.
+        etrans; first apply incl2.
+        solve_view_le. }
+      rewrite monPred_at_big_sepM.
+      setoid_rewrite monPred_at_sep.
+      setoid_rewrite monPred_at_embed.
+      simpl.
+      iFrame "physHist".
+      Unshelve. done.
+  Qed.
+
+  Lemma wp_load_at_simple ℓ sI Q prot `{!ProtocolConditions prot} st E :
+      {{{
+        ℓ ↦_AT^{prot} [sI] ∗
+        <obj> (∀ sL vL, ⌜ sI ⊑ sL ⌝ -∗ prot.(p_read) sL vL -∗ Q sL vL ∗ prot.(p_read) sL vL)
+      }}}
+        !_AT #ℓ @ st; E
+      {{{ sL vL, RET vL;
+        ℓ ↦_AT^{prot} [sL] ∗
+        <fence> (Q sL vL) }}}.
+    Proof.
+      iIntros (Φ) "[pts impl] post".
+      iApply (wp_load_at _ [] _ (λ v, Q sI v) Q with "[$pts impl]").
+      { iSplit.
+        * iIntros (??).
+          iExists True%I, _, _.
+          iIntros (?).
+          iSplitL ""; first naive_solver.
+          iIntros "_".
+          iApply (monPred_objectively_mono with "impl").
+          iIntros "impl P".
+          iApply ("impl" with "[//] P").
+        * iIntros (???).
+          iExists True%I, _, _.
+          iIntros (?).
+          iSplitL ""; first naive_solver.
+          iIntros "_".
+          iApply (monPred_objectively_mono with "impl").
+          iIntros "impl P".
+          iApply ("impl" with "[//] P"). }
+      iNext.
+      iIntros (?).
+      iIntros "[L|R]".
+      - iDestruct "L" as (?) "[pts Q]".
+        iApply "post".
+        iFrame "Q".
+        iApply mapsto_at_drop.
+        done.
+      - iApply "post".
+        iApply "R".
+    Qed.
+
+  (* Load a location where the protocol invariant is persistent. *)
+  Lemma wp_load_at_simple_pers ℓ (sI : ST) prot `{!ProtocolConditions prot} st E
+    `{∀ s v, Persistent (prot.(p_read) s v)} :
+      {{{ ℓ ↦_AT^{prot} [sI] }}}
+        !_AT #ℓ @ st; E
+      {{{ sL vL, RET vL;
+        ⌜ sI ⊑ sL ⌝ ∗ ℓ ↦_AT^{prot} [sL] ∗ <fence> (prot.(p_read) sL vL) }}}.
+  Proof.
+    iIntros (Φ) "pts Φpost".
+    iApply (wp_load_at_simple _ _
+      (λ s v, ⌜ sI ⊑ s ⌝ ∗ prot.(p_read) s v)%I with "[$pts]").
+    { iModIntro. iIntros (??) "$ #$". }
+    iNext.
+    iIntros (sL vL) "(pts & (>eq & hi))".
+    iApply "Φpost".
+    iFrame.
+  Qed.
+
+  (* Definition open_subjective (I P : dProp Σ) := <obj> I -∗ P ∗ I. *)
+
+  (* This is a load lemma that allows for a sort of "threading" of resources
+   * though all the invariants. The idea has some flaws (the order is arbitrary
+   * for instance) but maybe it can be used to come up witha stronger load lemma. *)
+  (* Lemma wp_load_at_strong ℓ ss s (QS : list (val → dProp Σ)) Q1 Q2 *)
+  (*   prot `{!ProtocolConditions prot} st E : *)
+  (*   length QS = length ss → *)
+  (*   {{{ *)
+  (*     ℓ ↦_AT^{prot} (ss ++ [s]) ∗ *)
+  (*     (* Based on all the existing writes we can show [Q1]. *) *)
+  (*     ((∀ vs, *)
+  (*       ([∗ list] i ↦ s; v ∈ ss ++ [s];vs, ∃ Q Q', *)
+  (*         ⌜ QS !! i = Some Q ⌝ -∗ *)
+  (*         ⌜ (QS ++ [Q1]) !! (S i) = Some Q' ⌝ -∗ *)
+  (*         <obj> prot.(p_inv) s v -∗ Q v -∗  prot.(p_inv) s v ∗ Q' v)) ∧ *)
+  (*     (* In case of a new write we can show [Q2] *) *)
+  (*     <obj> (∀ v v' s', *)
+  (*       ⌜ s ⊑ s' ⌝ -∗ *)
+  (*       prot.(p_inv) s' v -∗ *)
+  (*       Q1 v -∗ *)
+  (*       prot.(p_inv) s' v' ∗ Q2 s' v')) *)
+  (*   }}} *)
+  (*     !_AT #ℓ @ st; E *)
+  (*   {{{ v, RET v; *)
+  (*     (∃ s', ℓ ↦_AT^{prot} (ss ++ [s] ++ [s']) ∗ <fence> Q2 s' v) ∨ *)
+  (*     <fence> Q1 v *)
+  (*   }}}. *)
+  (* Proof. Abort. *)
+End wp_at.
