src/high/weakestpre/at/prelude.v
@@ -1,0 +1,408 @@
+(* Common lemmas shared by most atomic operations *)
+From iris.proofmode Require Import proofmode monpred.
+From iris.algebra Require Import gset.
+From iris_named_props Require Import named_props.
+
+From self Require Import extra solve_view_le encode_relation map_extra view_slice ipm_tactics.
+
+From self.lang Require Import syntax tactics lemmas.
+
+From self.base Require Import generational_resources primitive_laws.
+
+From self.high Require Import wrappers monpred_simpl protocol locations crash_weakestpre weakestpre.
+From self.high.modalities Require Import post_fence_sync_advanced.
+From self.high.lib Require Import abstract_state increasing_map.
+
+From self Require Export lang.
+From self.high Require Export dprop.
+
+Set Default Proof Using "Type*".
+
+Section wp_at.
+  Context `{AbstractState ST}.
+  Context `{!nvmBaseGS Σ Ω, !nvmHighGS Σ Ω, PerennialG Σ}.
+
+  Implicit Types (ℓ : loc) (σ : ST) (prot : LocationProtocol ST).
+  
+  (* These are specialized definitions for atomic locations. *)
+  Definition at_encoded_full_read_predicates_hold
+    (abs_hist: gmap time positive) (phys_hist: gmap time message)
+    offset (encp_full encp_read: enc_predicate) : iProp Σ :=
+      (* The predicate holds for "exclusive-write" message in the history. *)
+      ([∗ map] t ↦ msg; encS ∈ phys_hist; abs_hist,
+         if (decide (offset ≤ t ∧ phys_hist !! (S t) = None)) then (* full predicate *)
+           encoded_predicate_holds
+             encp_full
+             encS
+             msg.(msg_val)
+             (msg.(msg_store_view), msg.(msg_persisted_after_view), ∅)
+         else (* read predicate *)
+           encoded_predicate_holds
+             encp_read
+             encS
+             msg.(msg_val)
+             (msg.(msg_store_view), msg.(msg_persisted_after_view), ∅)).
+
+  (* It's still more hassle to replace [global_pview] with thread local version. *)
+  Definition at_encoded_pers_predicate_holds
+    ℓ (abs_hist: gmap time positive) (phys_hist: gmap time message)
+    (pview: option nat) (offset: nat) (encp_pers: enc_predicate): iProp Σ :=
+    ∃ (t: nat) encσ msg,
+      ⌜ abs_hist !! t = Some encσ ⌝ ∗
+      ⌜ phys_hist !! t = Some msg ⌝ ∗
+      (* if a location has never been [fence_sync]ed, it will not have any [persisted] knowledge,
+       * in which case we can always use [offset] *)
+      ⌜ Nat.add offset (default 0 pview) = t ⌝ ∗
+      (* It's easier to work with a per-location assertion. *)
+      default emp (persisted_loc ℓ <$> pview) ∗            
+      (* [p_pers] are objective anyway, might as well make it easy here. *)
+      encoded_predicate_holds encp_pers encσ msg.(msg_val) (∅, ∅, ∅).
+  
+  Definition loc_info ℓ prot encp_full encp_read encp_pers phys_hists phys_hist abs_hist offset pview : iProp Σ :=
+    "physHists" ∷ auth_map_map_auth phy_history_name phys_hists ∗
+    "%physHistsLook" ∷ ⌜ phys_hists !! ℓ = Some phys_hist ⌝ ∗
+    "%domEq" ∷ ⌜ dom phys_hist = dom abs_hist ⌝ ∗
+    "%increasing" ∷ ⌜ increasing_map (encode_relation (⊑@{ST})) abs_hist ⌝ ∗
+    "%atInvs" ∷
+      ⌜ map_Forall (λ t msg, atomic_loc_inv ℓ t msg) (drop_prefix phys_hist offset) ⌝ ∗
+    "#predFullEquiv" ∷ ▷ (encp_full ≡ encode_predicate (p_full prot)) ∗
+    "#predReadEquiv" ∷ ▷ (encp_read ≡ encode_predicate (p_read prot)) ∗
+    "#predPersEquiv" ∷ ▷ (encp_pers ≡ encode_predicate (p_pers prot)) ∗
+    "#frags" ∷ ([∗ map] t ↦ encσ ∈ abs_hist, frag_entry bumpers_name abs_history_name ℓ t encσ) ∗
+    "predFullReadHolds" ∷ at_encoded_full_read_predicates_hold abs_hist phys_hist offset encp_full encp_read ∗
+    "predPersHolds" ∷ at_encoded_pers_predicate_holds ℓ abs_hist phys_hist pview offset encp_pers ∗
+    "#predFullReadSplit" ∷ (∀ encσ v TV, ■ (encoded_predicate_holds encp_full encσ v TV -∗ encoded_predicate_holds encp_read encσ v TV)) ∗
+    "fullHist" ∷ know_full_encoded_history_loc ℓ 1 abs_hist ∗
+    "pts" ∷ ℓ ↦fh phys_hist.
+
+  Definition insert_impl ℓ encp_full encp_read encp_pers phys_hists phys_hist abs_hist offset pview: iProp Σ :=
+    ∀ t (σ: ST) encσ msg,
+      ⌜ offset ≤ t ⌝ -∗
+      ⌜ encode σ = encσ ⌝ -∗
+      ⌜ phys_hist !! t = None ⌝ -∗
+      ⌜ msg_store_view msg !!0 ℓ = t - offset ⌝ -∗
+      ⌜ msg_persist_view msg = msg_persisted_after_view msg ⌝ -∗
+      auth_map_map_auth phy_history_name phys_hists -∗
+      at_encoded_full_read_predicates_hold (<[ t := encσ ]>abs_hist) (<[ t := msg ]>phys_hist) offset encp_full encp_read -∗
+      at_encoded_pers_predicate_holds ℓ (<[ t := encσ ]> abs_hist) (<[ t := msg ]>phys_hist) pview offset encp_pers -∗
+      know_full_encoded_history_loc ℓ 1 abs_hist -∗
+      ⌜ increasing_map (encode_relation (⊑@{ST})) (<[ t := encσ ]>abs_hist) ⌝ -∗
+      ℓ ↦fh (<[t := msg ]> phys_hist) ==∗
+      know_frag_history_loc ℓ t σ ∗
+      auth_map_map_frag_singleton phy_history_name ℓ t msg ∗
+      interp.
+
+  Definition lookup_impl ℓ encp_full encp_read encp_pers phys_hists phys_hist abs_hist offset pview: iProp Σ :=
+    auth_map_map_auth phy_history_name phys_hists -∗
+    at_encoded_full_read_predicates_hold abs_hist phys_hist offset encp_full encp_read -∗
+    at_encoded_pers_predicate_holds ℓ abs_hist phys_hist pview offset encp_pers -∗
+    know_full_encoded_history_loc ℓ 1 abs_hist -∗
+    ℓ ↦fh phys_hist -∗
+    interp.
+
+  (* Get all information inside [interp] related to the location [ℓ]. *)
+  Lemma interp_get_at_loc ℓ prot offset TV :
+    interp -∗
+    is_at_loc ℓ -∗
+    know_protocol ℓ prot TV -∗
+    offset_loc ℓ offset -∗
+    ∃ phys_hists phys_hist (abs_hist : gmap nat positive) encp_full encp_read encp_pers pview,
+      loc_info ℓ prot encp_full encp_read encp_pers phys_hists phys_hist abs_hist offset pview ∗
+      (insert_impl ℓ encp_full encp_read encp_pers phys_hists phys_hist abs_hist offset pview ∧
+        lookup_impl ℓ encp_full encp_read encp_pers phys_hists phys_hist abs_hist offset pview).
+  Proof.
+    iNamed 1.
+    iIntros "isAt".
+    rewrite know_protocol_unfold.
+    iNamed 1.
+    iIntros "offset".
+    iDestruct (own_all_full_preds_pred with "full_predicates knowFullPred")
+      as (encp_full encPFullLook) "#encPFullEquiv".
+    iDestruct (own_all_read_preds_pred with "read_predicates knowReadPred")
+      as (encp_read encPReadLook) "#encPReadEquiv".
+    iDestruct (own_all_pers_preds_pred with "pers_predicates knowPersPred")
+      as (encp_pers ecpPPersLook) "#encPPersEquiv".
+    (* iDestruct (full_map_frag_singleton_agreee with "history hist") *)
+    (*   as %(absHist & enc & absHistLook & lookTS & decodeEnc). *)
+    (* iDestruct (big_sepM2_dom with "oldViewsDiscarded") as %offsetsDom. *)
+    iDestruct (offset_loc_offset_auth_agree with "offset offsets") as %offsetLook.
+    iDestruct (location_sets_singleton_included with "atLocs isAt") as %ℓSh.
+
+    iDestruct (big_sepM2_dom with "predsFullReadHold") as %domPhysHistEqAbsHist.
+    assert (is_Some (abs_hists !! ℓ)) as [abs_hist absHistLook].
+    { rewrite -elem_of_dom. set_solver. }
+    assert (is_Some (phys_hists !! ℓ)) as [phys_hist physHistsLook].
+    { rewrite -elem_of_dom domPhysHistEqAbsHist elem_of_dom. done. }
+
+    assert (na_views !! ℓ = None) as naViewLook. { apply not_elem_of_dom. set_solver. }
+
+    iDestruct (big_sepM2_delete with "predsFullReadHold") as "[predFullReadHolds allPredsFullReadHold]";
+      [done|done|].
+    iDestruct "predFullReadHolds" as (encp_full' encp_read' offset' ? ? ?) "predFullReadHolds".
+    simplify_map_eq.
+
+    iDestruct (big_sepM2_delete with "predsPersHold") as "[predPersHolds allPredsPersHold]";
+      [done|done|].
+    iEval (rewrite /encoded_pers_predicate_holds /lookup_zero) in "predPersHolds".
+    set (pview := global_pview !! ℓ).
+    iDestruct "predPersHolds" as (encp_pers' t_p offset' encσ_p msg_p ? ? ? ? ?) "[HpviewTemp predPersHolds]".
+
+    (* TODO: Maybe have a typeclass to make this assertion persistent? *)
+    iAssert  (□ (default emp (persisted_loc ℓ <$> (max_nat_car <$> pview))))%I  with "[HpviewTemp]" as "#Hpview".
+    { destruct pview; last done.
+      simpl.
+      by iDestruct "HpviewTemp" as "#?". }
+    iClear "HpviewTemp".
+    simplify_map_eq.
+    
+    iDestruct (big_sepM2_delete_l with "ordered")
+      as (order) "(%ordersLook & %increasingMap & #ordered2)";
+      first apply absHistLook.
+
+    iDestruct (orders_lookup with "allOrders knowPreorder") as %orderEq;
+      first apply ordersLook.
+    rewrite orderEq in increasingMap.
+
+    iDestruct (big_sepM2_dom with "predFullReadHolds") as %domEq.
+
+    (* We can now get the points-to predicate and execute the load. *)
+    iDestruct (big_sepM_delete with "ptsMap") as "[pts ptsMap]".
+    { naive_solver. }
+
+    eassert _ as invs.
+    { eapply map_Forall_lookup_1; first apply mapShared.
+      apply restrict_lookup_Some_2; last done.
+      apply map_lookup_zip_with_Some.
+      eexists _, _. split_and!; done. }
+    simpl in invs.
+
+    iDestruct (big_sepM_delete with "atLocsHistories") as
+      "(fullHist & atLocsHistories)".
+    { apply restrict_lookup_Some_2; done. }
+
+    iDestruct (big_sepM_lookup with "historyFragments") as "#histFrags"; first done.
+
+    iExists phys_hists, phys_hist, abs_hist, encp_full, encp_read, encp_pers, (max_nat_car <$> pview).
+    (* Give resources. *)
+    Opaque insert_impl lookup_impl.
+    iFrame (domEq increasingMap). iFrame (invs).
+    iFrame "encPFullEquiv".
+    iFrame "encPReadEquiv".
+    iFrame "encPPersEquiv".
+    iFrame "predFullReadHolds".
+    iFrame "histFrags".
+    iFrame "physHists".
+    iFrame "pts".
+    iFrame "fullHist".
+    rewrite -bi.sep_assoc. iSplitPure; first apply physHistsLook.
+    rewrite -bi.sep_assoc. iSplitL "predPersHolds".
+    { iExists _, encσ_p, msg_p. by iFrame "∗#". }
+    iSplit.
+    { iPoseProof (big_sepM2_lookup with "predFullReadSplit") as "split";
+        [ done | done | ].
+      iAssumption. }
+    (* We show the two different implications. *)
+    iSplit.
+    { Transparent insert_impl.
+      (* Get back resources. *)
+      iIntros (t_i σ encσ msg HAfterOffset Hencodeσ HphysLook HMsgStoreViewLook HMsgPersistViewLook)
+        "physHists predFullReadHolds predPersHolds fullHist order pts".
+
+      assert (abs_hist !! t_i = None)%I as HAbsHistLookNone.
+      { apply not_elem_of_dom. rewrite -domEq. apply not_elem_of_dom. done. }
+
+      iMod (full_map_full_entry_insert _ _ _ _ _ encσ with "history fullHist")
+        as "(history & fullHist & #histFrag)"; first done.
+
+      iDestruct (big_sepM_insert_delete with "[$atLocsHistories $fullHist]")
+        as "atLocsHistories".
+      iDestruct (big_sepM_insert_delete with "[$ptsMap $pts]") as "ptsMap".
+
+      iPoseProof (big_sepM2_insert_delete with "[$allPredsFullReadHold predFullReadHolds]")
+        as "allPredsFullReadHold".
+      { iExists encp_full, encp_read, offset. rewrite naViewLook. iFrame. done. }
+      iPoseProof (big_sepM2_insert_delete _ _ _ _ (<[t_i:=msg]> phys_hist) (<[t_i:=encσ]> abs_hist) with "[$allPredsPersHold predPersHolds]")
+        as "allPredsPersHold".
+      { iExists encp_pers, _, offset, encσ_p, msg_p.
+        assert ((offset + default 0 (max_nat_car <$> pview)) ≠ t_i) by congruence.
+        iDestruct "predPersHolds" as (t_p encσ_p' msg_p' ? ? ? ) "(Hpview' & predPersHolds)".
+        assert (msg_p = msg_p') as <- by (by simplify_map_eq).
+        assert (encσ_p = encσ_p') as <- by (by simplify_map_eq).
+        iFrame.
+        rewrite ?lookup_insert_ne //. }
+      iMod (auth_map_map_insert with "physHists") as "(physHists & _ & physHistFrag)"; [try done|try done|].
+
+      iDestruct (big_sepM2_insert_delete with "[$ordered2 $order]") as "ordered3".
+      rewrite (insert_id orders). (* last congruence. *)
+      2: { rewrite ordersLook. f_equal.
+          rewrite orderEq.
+          reflexivity. }
+
+      iDestruct (bumpers_lookup with "allBumpers knowBumper") as %bumpersLook.
+
+      iModIntro.
+      iSplit; first (iApply frag_history_equiv; rewrite -Hencodeσ; iFrame "histFrag").
+      iFrameF "physHistFrag".
+      (* We re-establish [interp]. *)
+      iExistsN.
+      iFrameNamedF.
+      iSplitPure; first set_solver.
+      iFrameNamedF.
+      iFrame "allOrders".
+      iFrame "ordered3".
+      iFrame "allPredsFullReadHold allPredsPersHold".
+      iFrame "full_predicates read_predicates pers_predicates".
+      iFrame "atLocs".
+      iFrame "naView naLocs allBumpers bumpMono".
+      (* historyFragments *)
+      iSplit.
+      { iApply (big_sepM_insert_2 with "[] historyFragments").
+        iApply (big_sepM_insert_2 with "histFrag []").
+        iApply (big_sepM_lookup with "historyFragments").
+        done. }
+      (* [locsDisjoint] *)
+      iSplitPure; first apply locsDisjoint.
+      (* [histDomLocs] *)
+      iSplit. { iPureIntro. set_solver. }
+      (* [naViewsDom] *)
+      iSplitPure; first done.
+      (* [mapShared] - We need to show that the newly inserted message satisfied *)
+      (* the restriction on shared locations that their persist view and their *)
+      (* persisted after view is equal. *)
+      iSplit.
+      { iPureIntro.
+        erewrite <- (insert_id offsets); last done.
+        rewrite -map_insert_zip_with.
+        setoid_rewrite (restrict_insert ℓ); last done.
+        rewrite /shared_locs_inv.
+        apply Nat.le_exists_sub in HAfterOffset as (tE & -> & ?).
+        rewrite -drop_prefix_insert.
+        apply map_map_Forall_insert_2.
+        - apply restrict_lookup_Some_2; last done.
+          apply map_lookup_zip_with_Some. naive_solver.
+        - simpl.
+          rewrite /atomic_loc_inv.
+          split; last done.
+          rewrite HMsgStoreViewLook. lia.
+        - done. }
+      iSplitL "atLocsHistories".
+      {
+        rewrite /know_full_encoded_history_loc.
+        (* NOTE: This rewrite is mega-slow. *)
+        iEval (setoid_rewrite (restrict_insert ℓ at_locs (<[t_i:=encσ]> abs_hist) abs_hists ℓSh)).
+        iFrame. }
+      (* [histPViewDoms] *)
+      iSplitPure. etrans; [ done | apply dom_insert_subseteq].
+      (* [FullBumpersDoms] *)
+      iSplitPure; first done.
+      (* [ReadBumpersDoms] *)
+      iSplitPure; first done.
+      (* [PersBumpersDoms] *)
+      iSplitPure; first done.
+      (* iFrameF "predFullPostCrash". *)
+      iSplit; first iAssumption.
+      iSplit; first iAssumption.
+      iFrame (bumperBumpToValid).
+      (* "bumperSome" *)
+      iApply (big_sepM2_update_left with "bumperSome"); eauto.
+      iPureIntro. intros bumperSome.
+      apply map_Forall_insert_2; eauto.
+      rewrite /encode_bumper. rewrite -Hencodeσ decode_encode. done. }
+    (* [lookup_impl] *)
+    { Transparent lookup_impl.
+      iIntros "physHists predFullReadHolds predPersHolds fullHist pts".
+      iDestruct (big_sepM_insert_delete with "[$atLocsHistories $fullHist]")
+        as "atLocsHistories".
+      iDestruct (big_sepM_insert_delete with "[$ptsMap $pts]") as "ptsMap".
+      iDestruct (big_sepM2_insert_delete with "[$ordered2]") as "ordered3";
+        first done.
+      iDestruct (big_sepM2_insert_delete with "[$allPredsFullReadHold predFullReadHolds]")
+        as "predsFullReadHold".
+      { iExistsN. rewrite naViewLook. iFrame "predFullReadHolds". done. }
+      iDestruct (big_sepM2_insert_delete with "[$allPredsPersHold predPersHolds]")
+        as "predsPersHold".
+      { iExistsN.
+        iDestruct "predPersHolds" as (? ? ? ? ? ?) "[Hpview' predPersHolds]".
+        simplify_map_eq.
+        iFrame.
+        done. }
+      rewrite (insert_id orders); last congruence.
+      rewrite (insert_id phys_hists); last congruence.
+      rewrite (insert_id abs_hists); last congruence.
+      rewrite (insert_id (restrict at_locs abs_hists)).
+      2: { apply restrict_lookup_Some_2; done. }
+
+      (* We re-establish [interp]. *)
+      iExistsN.
+      iFrameNamedF.
+      iSplit; first iAssumption.
+      iSplit; first iAssumption.
+      iFrame "bumperSome".
+      done. }
+  Qed.
+
+    Lemma read_atomic_location_no_inv t_i t_l (physHist : history) absHist vm SVm FVm
+        PVm ℓ (e_i : positive) (s_i : ST) :
+    t_i ≤ t_l →
+    dom physHist = dom absHist →
+    absHist !! t_i = Some e_i →
+    decode e_i = Some s_i →
+    increasing_map (encode_relation (⊑@{ST})) absHist →
+    physHist !! t_l = Some (Msg vm SVm FVm PVm) →
+    ∃ s_l e_l,
+      absHist !! t_l = Some e_l ∧
+      decode e_l = Some s_l ∧
+      (* SVm !!0 ℓ = t_l ∧ *)
+      (* FVm = PVm ∧ *)
+      s_i ⊑ s_l.
+  Proof.
+    intros le domEq ? decodeEnc ? ?.
+    assert (is_Some (absHist !! t_l)) as (e_l & ?).
+    { apply elem_of_dom. rewrite <- domEq. apply elem_of_dom. naive_solver. }
+    (* The loaded state must be greater than [s_i]. *)
+    assert (encode_relation (⊑@{ST}) e_i e_l) as orderRelated.
+    { eapply increasing_map_increasing_base; try done.
+      rewrite /encode_relation. rewrite decodeEnc. simpl. done. }
+    epose proof (encode_relation_inv _ _ _ orderRelated)
+      as (? & s_l & eqX & decodeS' & s3InclS').
+    assert (x = s_i) as -> by congruence.
+   exists s_l, e_l. done.
+  Qed.
+  
+  Lemma read_atomic_location t_i t_l offset (physHist : history) absHist vm SVm FVm
+        PVm ℓ (e_i : positive) (s_i : ST) :
+    t_i ≤ t_l →
+    offset ≤ t_l →
+    dom physHist = dom absHist →
+    absHist !! t_i = Some e_i →
+    decode e_i = Some s_i →
+    increasing_map (encode_relation (⊑@{ST})) absHist →
+    map_Forall (λ (t : nat) (msg : message), atomic_loc_inv ℓ t msg)
+               (drop_prefix physHist offset) →
+    physHist !! (t_l) = Some (Msg vm SVm FVm PVm) →
+    ∃ s_l e_l,
+      absHist !! (t_l) = Some e_l ∧
+      decode e_l = Some s_l ∧
+      SVm !!0 ℓ = t_l - offset ∧
+      FVm = PVm ∧
+      s_i ⊑ s_l.
+  Proof.
+    intros le le' domEq ? decodeEnc ? atInvs ?.
+    eassert _ as temp.
+    { replace t_l with ((t_l - offset) + offset) in H4 by lia.
+      eapply map_Forall_lookup_1; first apply atInvs.
+      rewrite drop_prefix_lookup.
+      done. }
+    rewrite /atomic_loc_inv /= in temp. destruct temp as [SV'lookup <-].
+    assert (is_Some (absHist !! (t_l))) as (e_l & ?).
+    { apply elem_of_dom. rewrite <- domEq. apply elem_of_dom. naive_solver. }
+    (* The loaded state must be greater than [s_i]. *)
+    assert (encode_relation (⊑@{ST}) e_i e_l) as orderRelated.
+    { eapply (increasing_map_increasing_base _ _ t_i t_l); try (done || lia).
+      rewrite /encode_relation. rewrite decodeEnc. simpl. done. }
+    epose proof (encode_relation_inv _ _ _ orderRelated)
+      as (? & s_l & eqX & decodeS' & s3InclS').
+    assert (x = s_i) as -> by congruence.
+   exists s_l, e_l. done.
+  Qed.
+End wp_at.
