src/high/weakestpre/at/store.v
@@ -1,0 +1,374 @@
+From iris.proofmode Require Import proofmode monpred.
+From iris.algebra Require Import gset.
+From iris_named_props Require Import named_props.
+
+From self Require Import extra solve_view_le encode_relation map_extra view_slice.
+
+From self.lang Require Import syntax tactics lemmas.
+
+From self.base Require Import generational_resources primitive_laws.
+
+From self.high Require Import wrappers monpred_simpl protocol locations crash_weakestpre weakestpre.
+From self.high.modalities Require Import post_fence_sync_advanced.
+From self.high.lib Require Import abstract_state increasing_map.
+From self.high.weakestpre.at Require Import prelude.
+
+From self Require Export lang.
+From self.high Require Export dprop.
+
+Set Default Proof Using "Type*".
+
+Section wp_at.
+  Lemma wp_store_at ℓ prot ss s_i s_t v_t st E `{!ProtocolConditions prot} :
+    {{{
+      ℓ ↦_AT^{prot} (ss ++ [s_i]) ∗
+      prot.(p_full) s_t v_t ∗
+      (* NOTE: This does _not_ work. *)
+      (* "phi" ∷ (∀ v_i, ϕ s_i v_i _ -∗ ϕ s_t v_t _ ∗ ϕ s_i v_i _) ∗ *)
+      (* NOTE: This should work and be more general. *)
+      (* "phi" ∷ (∀ v_i, (<obj> (ϕ s_i v_i -∗ ϕ s_i_v ∗ R)) ∗ (R -∗ ϕ s_t v_t)) ∗ *)
+      ⌜ s_i ⊑ s_t ⌝ ∗
+      (* The new state must be concurrent with possible other states. *)
+      (∀ v_i s_c v_c, ⌜ s_i ⊑ s_c ⌝ -∗
+        (* NOTE: We could give predicates for all states in ss here. *)
+        prot.(p_read) s_i v_i ∗ prot.(p_full) s_t v_t ∗ prot.(p_read) s_c v_c -∗
+          ⌜ s_t ⊑ s_c ∧ s_c ⊑ s_t ⌝)
+    }}}
+      #ℓ <-_AT v_t @ st; E
+    {{{ RET #(); ℓ ↦_AT^{prot} ((ss ++ [s_i]) ++ [s_t]) }}}.
+  Proof.
+    intros Φ.
+    iModel.
+    iIntros "(pts & phi & %targetGt & greater)".
+    iDestruct "pts" as (abs_hist phys_hist tLo t_i offset s' ms) "H". iNamed "H".
+    iDestruct "tSLe" as %tSLe.
+    (* iDestruct (store_lb_protocol with "storeLb") as "#knowProt". *)
+    iDestruct (know_protocol_extract with "locationProtocol")
+      as "(#knowPred & #knowPreorder & #knowBumper)".
+    rewrite -know_protocol_unfold.
+
+    rewrite /store_lb.
+    (* iDestruct "storeLb" as (t_i offset) "(#prot & #hist & #offset & %tSLe)". *)
+    (* We unfold the WP. *)
+    iIntros ([TV' ?] [incl [= <-]]) "Φpost".
+    (* iIntros (TV' incl) "Φpost". *)
+    iApply wp_unfold_at.
+    iIntros ([[SV PV] BV] incl2) "#val".
+
+    iApply wp_extra_state_interp. { done. }
+    { apply prim_step_store_rel_no_fork. }
+
+    iIntros "interp".
+    rewrite /is_at_loc /offset_loc 2!lift_d_at.
+    iDestruct (interp_get_at_loc with "interp isAtLoc locationProtocol offset")
+      as (physHists physHist absHist predFull predRead predPers tP) "(R & [reins _])".
+    iNamed "R".
+
+    (* We add this to prevent Coq from trying to use [highExtraStateInterp]. *)
+    set (extra := (Build_extraStateInterp _ _)).
+    iApply wp_fupd.
+
+    iApply (wp_store_release with "[$pts $val]").
+    iIntros "!>" (t_t) "(%look & %gt & #valNew & pts)".
+    simpl in gt.
+    simpl in tSLe.
+    rewrite drop_prefix_lookup in look.
+
+    (* We can conclude that [t_t] is strictly greater than [t_i]. *)
+    assert (t_i - offset < t_t) as tILtTt.
+    { destruct TV as [[??]?].
+      destruct TV' as [[??]?].
+      destruct incl as [[??]?].
+      destruct incl2 as [[??]?].
+      eapply Nat.le_lt_trans; last done.
+      etrans; first done.
+      f_equiv.
+      etrans; done. }
+    assert (t_i < t_t + offset) as ? by lia.
+
+    iFrame "valNew".
+
+    assert (abs_hist !! t_i = Some s_i).
+    { eapply map_sequence_lookup_hi in slice.
+      rewrite last_snoc in slice.
+      apply slice. }
+    rewrite monPred_at_big_sepM.
+    iDestruct (big_sepM_lookup with "absHist") as "hist"; first done.
+
+    rewrite /know_frag_history_loc_d lift_d_at.
+    iDestruct (history_full_entry_frag_lookup with "fullHist hist") as %look'.
+    destruct look' as (e_i & absHistLook' & hip).
+    assert (is_Some (physHist !! t_i)) as [vI physHistLook].
+    { rewrite -elem_of_dom domEq elem_of_dom. done. }
+
+    (* We must extract the phi for the initial state from "phi". *)
+
+    iPoseProof (big_sepM2_sep_2 with "predFullHolds predReadHolds") as "predHolds".
+    iDestruct (big_sepM2_delete with "predHolds") as "[phiI predHolds]";
+      [apply physHistLook | done | ].
+
+    iAssert (
+      ⌜increasing_map (encode_relation sqsubseteq) (<[(t_t+offset)%nat:=encode s_t]> absHist)⌝
+                      )%I as %incri.
+    { iApply (bi.pure_mono).
+      { apply
+         (increasing_map_insert_after _ _ _ _ _ (encode s_t) increasing
+                                      absHistLook'); last done.
+        eapply encode_relation_decode_iff; eauto using decode_encode. }
+      iIntros (t_c e_c ? iLeC).
+
+      iAssert (p_read prot s_i (memory.msg_val vI)
+                 (memory.msg_store_view vI,
+                    memory.msg_persisted_after_view vI,
+                      ∅, gnames))%I with "[phiI]" as "phiI". {
+        destruct (decide (offset ≤ t_i ∧ physHist !! S t_i = None)) as [ [] | no ].
+        - iDestruct ("phiI") as "[phiI _]".
+          iSpecialize ("phiI" with "[%] [//]"); first lia.
+          iDestruct (predicate_holds_phi_decode with "predFullEquiv phiI") as "phiI";
+            first done.
+          iPoseProof (full_read_split with "phiI") as "[phiI _]".
+          iFrame.
+        - iDestruct ("phiI") as "[_ phiI]".
+          rewrite not_and_l in no.
+          iSpecialize ("phiI" with "[%]").
+          { destruct no; [ left; lia | right; by destruct (_ !! S t_i) ]. }
+          iDestruct (predicate_holds_phi_decode with "predReadEquiv phiI") as "phiI";
+            first done.
+          iFrame.
+      }
+
+      assert (is_Some (physHist !! t_c)) as [[????] look2].
+      { rewrite -elem_of_dom domEq elem_of_dom. done. }
+
+      eassert _ as  temp. { eapply (read_atomic_location_no_inv t_i t_c); done || lia. }
+      destruct temp as (s_c & encSC & ? & decodeS' & orderRelated).
+      simplify_eq.
+      rewrite /encode_relation. rewrite decode_encode. rewrite decodeS'.
+
+      iDestruct (big_sepM2_delete with "predHolds") as "[phiC predHolds]";
+        [ rewrite lookup_delete_ne; [ apply look2 | lia ] |
+          rewrite lookup_delete_ne; [ done | lia ] | ].
+
+      iAssert (p_read prot s_c msg_val
+                 (msg_store_view, msg_persisted_after_view, ∅, gnames))%I
+        with "[phiC]" as "phiC". {
+        destruct (decide (offset ≤ t_c ∧ physHist !! S t_c = None)) as [ [] | no ].
+        - iDestruct ("phiC") as "[phiC _]".
+          iSpecialize ("phiC" with "[%] [//]"); first by lia.
+          iDestruct (predicate_holds_phi_decode with "predFullEquiv phiC") as "phiC";
+            first done.
+          iPoseProof (full_read_split with "phiC") as "[phiC _]".
+          iFrame.
+        - iDestruct ("phiC") as "[_ phiC]".
+          rewrite not_and_l in no.
+          iSpecialize ("phiC" with "[%]").
+          { destruct no; [ left; lia | right; by destruct (_ !! S t_c) ]. }
+          iDestruct (predicate_holds_phi_decode with "predReadEquiv phiC") as "phiC";
+            first done.
+          iFrame.
+
+     }
+
+      iSpecialize ("greater" $! _ s_c _).
+      iEval (monPred_simpl) in "greater".
+
+      iSpecialize ("greater" $! (TV, _) with "[%] [%]"); [done|done|].
+      iEval (monPred_simpl) in "greater".
+      iEval (setoid_rewrite monPred_at_pure) in "greater".
+
+      iApply ("greater" $! (TV' ⊔ (_) ⊔ (msg_to_tv vI), _)).
+      { iPureIntro. split; last done. etrans; first apply incl.
+        rewrite -assoc.
+        apply thread_view_le_l. }
+      monPred_simpl.
+      iFrame.
+      iSplitL "phiI".
+      { iApply monPred_mono; last iApply "phiI".
+        split; last done. apply thread_view_le_r. }
+      iSplitL "phi".
+      { iApply monPred_mono; last iApply "phi".
+        split; last done.
+        rewrite -assoc.
+        etrans; last apply thread_view_le_l. done. }
+
+      iApply monPred_mono; last iApply "phiC".
+      split; last done.
+      rewrite (comm _ TV').
+      rewrite -assoc.
+      apply thread_view_le_l. }
+
+    iDestruct (big_sepM2_insert_delete with "[phiI $predHolds]") as "predHolds";
+      first iFrame.
+    rewrite (insert_id physHist t_i); last done.
+    rewrite (insert_id absHist t_i); last done.
+
+    rewrite drop_prefix_insert.
+
+    iEval (rewrite big_sepM2_sep) in "predHolds".
+    iDestruct "predHolds" as "[predFullHolds predReadHolds]".
+    rewrite /insert_impl.
+
+    iMod ("reins" $! (t_t + offset) s_t
+      with "[%] [//] [//] [] [] [$] [predFullHolds phi predReadHolds] [predPersHolds] fullHist [//] pts")
+        as "(#frag & #physHistFrag & $)".
+    { lia. }
+    { iPureIntro. simpl.
+      replace (t_t + offset - offset) with t_t by lia.
+      apply lookup_zero_insert. }
+    { done. }
+    { rewrite -big_sepM2_sep.
+      iPoseProof (big_sepM2_sep_2 with "[$] [$]") as "predHolds".
+      iApply (big_sepM2_insert_2 with "[phi] [predHolds]").
+      { simpl.
+        iIntros.
+        rewrite lookup_insert_ne; last lia.
+        destruct (physHist !! S(t_t + offset)).
+        - iSplitL ""; first by iIntros.
+          iIntros.
+          iPoseProof (full_read_split with "phi") as "[phi _]".
+          rewrite /encoded_predicate_holds.
+          iExists (prot.(p_read) s_t v_t).
+          iSplit.
+          { iApply pred_encode_Some. done. }
+          destruct TV as [[??]?].
+          iDestruct (into_no_buffer_at with "phi") as "phi".
+          iApply monPred_mono; last iFrame.
+          destruct TV' as [[??]?].
+          repeat split; last done.
+          + simpl. etrans; first apply incl. etrans; first apply incl2.
+            apply view_insert_le'; [done|lia].
+          + simpl.
+            etrans; first apply incl.
+            apply incl2.
+        - iSplitR ""; last (iIntros ([ | contra ]);
+                            [lia | apply is_Some_None in contra; done]).
+          iIntros.
+          rewrite /encoded_predicate_holds.
+          iExists (prot.(p_full) s_t v_t).
+          iSplit.
+          { iApply pred_encode_Some. done. }
+          destruct TV as [[??]?].
+          iDestruct (into_no_buffer_at with "phi") as "phi".
+          iApply monPred_mono; last iFrame.
+          destruct TV' as [[??]?].
+          repeat split; last done.
+          + simpl. etrans; first apply incl. etrans; first apply incl2.
+            apply view_insert_le'; [done|lia].
+          + simpl.
+            etrans; first apply incl.
+            apply incl2.
+      }
+      { iApply (big_sepM2_impl with "predHolds").
+        simpl.
+        iIntros (t msg encS physHistLook'' absHistLook'') "!> H".
+        destruct (decide (offset ≤ t ∧ physHist !! S t = None)) as [ [] | no ].
+        - iDestruct "H" as "[_ H]".
+          destruct (decide (S t = t_t + offset)) as [-> | ?].
+          + rewrite lookup_insert.
+            iSplitL ""; first by iIntros.
+            iIntros.
+            iSpecialize ("H" with "[%] [//]"); first lia.
+            iSpecialize ("predFullReadSplit" with "H").
+            iFrame.
+          + rewrite lookup_insert_ne; last lia.
+            iSplitR ""; last (iIntros ([ | []]); [ lia | congruence ]).
+            iIntros.
+            iSpecialize ("H" with "[%] [//]"); first lia.
+            iFrame.
+        - iDestruct "H" as "[H _]".
+          rewrite not_and_l in no.
+          iSpecialize ("H" with "[%]").
+          { destruct no; [ left; lia | right; by destruct (_ !! S t) ]. }
+          iSplitL "".
+          + rewrite lookup_insert_None.
+            iIntros (? []).
+            destruct no; [ lia | congruence].
+          + iIntros.
+            iApply "H".
+    } }
+    { rewrite /encoded_pers_predicate_hold.
+      iDestruct "predPersHolds" as (encSP msgP) "(% & % & predPersHolds)".
+      assert (tP ≠ t_t + offset) by by simplify_map_eq.
+      iExists encSP, msgP.
+      do ? (rewrite lookup_insert_ne; last done).
+      iFrame.
+      done. }
+    (* We are done updating ghost state. *)
+    iModIntro.
+    iSplit. { iPureIntro. simpl. solve_view_le. }
+
+    iEval (rewrite monPred_at_wand) in "Φpost".
+    iApply "Φpost".
+    - iPureIntro. split; last done. solve_view_le.
+    - iExistsN.
+
+      iSplitPure. { rewrite last_snoc. reflexivity. }
+      iSplitPure. { eapply map_sequence_insert_snoc; done. }
+      iSplitPure.
+      { eapply map_sequence_insert_snoc; last done; first lia.
+        eapply map_no_later_dom; last apply nolater.
+        done. }
+      iSplitPure.
+      { eapply map_no_later_insert; last done. lia. }
+      iSplitPure.
+      { rewrite 2!dom_insert_L. rewrite absPhysHistDomEq. done. }
+      simpl.
+      iFrameF "isAtLoc".
+      rewrite big_sepM_insert. 2: { apply nolater. lia. }
+      rewrite big_sepM_insert.
+      2: {
+        eapply map_dom_eq_lookup_None; first done.
+        apply nolater. lia. }
+      rewrite -know_protocol_unfold.
+      iSplitL "locationProtocol".
+      { iApply view_objective_at. iFrame "locationProtocol". }
+      iSplitPure.
+      { apply: increasing_map_insert_last; done. }
+      iSplit.
+      { simpl. rewrite monPred_at_sep. simpl. iFrame "frag".
+        rewrite -monPred_at_big_sepM.
+        iApply view_objective_at.
+        rewrite monPred_at_big_sepM.
+        iEval (rewrite monPred_at_big_sepM).
+        simpl.
+        iFrame "absHist". }
+        rewrite monPred_at_big_sepM.
+      iFrame "offset".
+      iSplit; last first.
+      { simpl. iPureIntro.
+        rewrite lookup_zero_insert.
+        lia. }
+      simpl.
+      iSplit.
+      { simpl. iFrame "physHistFrag". solve_view_le. }
+      iEval (rewrite -monPred_at_big_sepM) in "physHist".
+      iApply monPred_mono; last iApply "physHist".
+      split; last done.
+      etrans; first apply incl.
+      etrans; first apply incl2.
+      repeat split; solve_view_le.
+  Qed.
+
+  (* Rule for store on an atomic. *)
+  (* Lemma wp_store_at_strong R Q ℓ ss s_i s_t v_t (prot : LocationProtocol ST) st E : *)
+  (*   {{{ *)
+  (*     ℓ ↦_AT^{prot} (ss ++ [s_i]) ∗ *)
+  (*     (* [s_l] is the state of the store that ours end up just after in the *)
+  (*     history. *) *)
+  (*     (∀ s_l v_l, ⌜ s_i ⊑ s_l ⌝ -∗ ∃ s_t, *)
+  (*       (* The state we picked fits in the history. *) *)
+  (*       (∀ v_i s_n v_n, ⌜ s_l ⊑ s_n ⌝ -∗ *)
+  (*         prot.(p_inv) s_i v_i -∗ *)
+  (*         prot.(p_inv) s_l v_l -∗ *)
+  (*         prot.(p_inv) s_n v_n -∗ *)
+  (*         ⌜ s_l ⊑ s_t ⌝ ∗ ⌜ s_t ⊑ s_n ⌝) ∧ *)
+  (*       (* Extract from the location we load. *) *)
+  (*       (<obj> (prot.(p_inv) s_l v_l -∗ prot.(p_inv) s_l v_l ∗ R s_l)) ∗ *)
+  (*       (* Establish the invariant for the value we store. *) *)
+  (*       (R s_l -∗ prot.(p_inv) s_t v_t ∗ Q s_t)) *)
+  (*   }}} *)
+  (*     #ℓ <-_AT v_t @ st; E *)
+  (*   {{{ RET #(); store_lb ℓ prot s_t ∗ Q s_t }}}. *)
+  (* Proof. *)
+  (* Abort. *)
+End wp_at.
